src/framework/framework.v
@@ -1,0 +1,744 @@
+Require Import Fin.
+Require Import PArray Init.Byte.
+Require Import framework.monad.
+
+(***************************************
+  Definition of core objects
+***************************************)
+
+Definition fin := Fin.t.
+
+Definition NodeSet (n : nat) := fin n.
+Definition Message := array byte.
+
+(***************************************
+  Definition of trace
+***************************************)
+
+(* Main action type, it describes a simple I/O interface *)
+Inductive IAction {I O : Type} :=
+  | ISend : O -> IAction
+  | IRecv : I -> IAction
+.
+
+(*
+
+An action of a node is :
+- either an frontend action (output something to the user/upper level protocol)
+- either a backend action (output something to the network/lower level protocol)
+
+For compatibility, we call IOutput and IInput the equivalent of ISend and IRecv
+to describe the frontend interface, where IInput is and input for the protocol
+and IOutput is an output of the protocol.
+
+*)
+Definition NodeAction {I O I' O'} := (@IAction I O + @IAction I' O')%type.
+
+Notation "'frontend'" := inl.
+Notation "'backend'" := inr.
+Notation "'IOutput'" := IRecv.
+Notation "'IInput'" := ISend.
+Notation "'Send' m" := (backend (ISend m)) (at level 100).
+Notation "'Recv' m" := (backend (IRecv m)) (at level 100).
+Notation "'Output' m" := (frontend (IOutput m)) (at level 100).
+Notation "'Input' m" := (frontend (IInput m)) (at level 100).
+
+(* The actions of a model are actions of nodes labeled with a node identifier n *)
+Definition ModelAction {I O I' O'} (n : nat) := (NodeSet n * @NodeAction I O I' O')%type.
+
+(* A trace is a sequence of actions *)
+Definition Trace (Action : Type) := nat -> option Action.
+
+(* TransformTrace is a simple wrapper to apply functions on traces *)
+Definition TransformTrace {A B : Type} (f : A -> option B) (t : Trace A) : Trace B :=
+  (fun i => match t i with
+           | Some a => f a
+           | None => @None B
+        end).
+
+(*
+  InvarientTrace states that the property P holds at every step of the trace,
+  NOTE : might have to improve the definition to take the history as an input for P ...
+ *)
+Definition InvarientTrace {A : Type} (P : A -> Prop) (t : Trace A) : Prop :=
+  forall i, match t i with
+         | Some a => P a
+         | _ => True
+      end.
+
+(* transform a trace on backend actions to a trace on model actions *)
+Definition InterfaceTraceAsBackend {I O I' O'} {n : nat} : Trace (NodeSet n * IAction)%type -> Trace (@ModelAction I O I' O' n) :=
+  TransformTrace (fun a => let '(p, node_act) := a in Some (p, backend node_act)).
+
+(* a specification is a property on actions *)
+Definition Specification (Action : Type) := Trace Action -> Prop.
+
+(* An interface is a specification of the behaviour of an interface with multiple nodes *)
+Definition Interface {I O} := forall i : nat, Specification (NodeSet i * @IAction I O)%type.
+
+(* project the trace on the actions of one node *)
+Definition ProjectTraceOnNode
+  {I O I' O'}
+  {n : nat}
+  (p : fin n) :
+  Trace (@ModelAction I O I' O' n) -> Trace (NodeAction) :=
+  TransformTrace (fun a => let '(_, node_act) := a in Some (node_act)).
+
+(* project the trace on the actions of the backend of the nodes *)
+Definition ProjectTraceOnBackend
+  {I O I' O'}
+  {n : nat} :
+  Trace (@ModelAction I O I' O' n) -> Trace (NodeSet n * IAction)%type :=
+  TransformTrace (
+      fun a => let '(p, node_act) := a in
+            match node_act with
+              | backend a' => Some (p, a')
+              | _ => None
+            end
+    ).
+
+(***************************************
+  Now we define a intermediaire
+  representation for the proofs :
+  The designer have to provide two
+  functions : a input handler (for the
+  external interface) and a recv handler
+  (for the backend interface)
+***************************************)
+
+Section local_representation.
+  Import monad.
+  Import Lia.
+
+  Variable InputType OutputType RecvType SendType : Type.
+  Variable State : Type.
+  Definition Handler := GenHandler SendType State OutputType unit.
+  Variable InputHandler : InputType -> Handler.
+  Variable RecvHandler : RecvType -> Handler.
+
+  (* We smash both inputs and recv types together *)
+  Definition input_types := (InputType+RecvType)%type.
+
+  Definition PreRun : Type := nat -> input_types.
+
+  (* This function compute a transition given an input *)
+  Definition compute_transition
+    (st : State)
+    (i : input_types) :=
+    match i with
+    | frontend q =>
+        runGenHandler_ignore st (InputHandler q)
+    | backend q =>
+        runGenHandler_ignore st (RecvHandler q)
+    end.
+
+  Require Import List.
+  Import ListNotations.
+
+  (* this is the model of a node of our current protocol *)
+  Definition SpecializedNodeModel :=
+    @NodeAction OutputType InputType RecvType SendType.
+
+  (* Transforms a list of inputs values into a list of input actions *)
+  Fixpoint out_to_model (out : list OutputType) : list SpecializedNodeModel :=
+    match out with
+    | [] => []
+    | a::b => (Output a)::(out_to_model b)
+    end.
+
+  (* Transforms a list of recv values into a list of recv actions *)
+  Fixpoint send_to_model snd : list SpecializedNodeModel :=
+    match snd with
+    | [] => []
+    | a::b => (Send a)::(send_to_model b)
+    end.
+
+  Lemma out_of_model_no_recv :
+    forall out, forall p, ~In (Recv p) (out_to_model out).
+  Proof.
+    induction out.
+    - intros. simpl. auto.
+    - intros. simpl. intro. destruct H. inversion H.
+      eapply IHout. apply H.
+  Qed.
+
+  Lemma send_to_model_no_recv :
+    forall out, forall p, ~In (Recv p) (send_to_model out).
+  Proof.
+    induction out.
+    - intros. simpl. auto.
+    - intros. simpl. intro. destruct H. inversion H.
+      eapply IHout. apply H.
+  Qed.
+
+  Lemma out_of_model_no_input :
+    forall out, forall p, ~In (Input p) (out_to_model out).
+  Proof.
+    induction out.
+    - intros. simpl. auto.
+    - intros. simpl. intro. destruct H. inversion H.
+      eapply IHout. apply H.
+  Qed.
+
+  Lemma send_to_model_no_input :
+    forall out, forall p, ~In (Input p) (send_to_model out).
+  Proof.
+    induction out.
+    - intros. simpl. auto.
+    - intros. simpl. intro. destruct H. inversion H.
+      eapply IHout. apply H.
+  Qed.
+
+  (* This local function create a list of action from an action and an input *)
+  Definition create_list_from_transition
+    (st : State)
+    (i : input_types) : State * list SpecializedNodeModel :=
+    match i with
+    | frontend q =>
+        let '(_out, st', _send) := runGenHandler_ignore st (InputHandler q) in
+        (st', (Input q)::(out_to_model _out) ++ (send_to_model _send))
+    | backend q =>
+        let '(_out, st', _send) := runGenHandler_ignore st (RecvHandler q) in
+        (st', (Recv q)::(out_to_model _out) ++ (send_to_model _send))
+    end.
+
+  Lemma create_list_from_transition_nth_recv :
+    forall st, forall i, forall n, forall p,
+      nth_error (snd (create_list_from_transition st i)) n = Some (Recv p) -> n = 0.
+  Proof.
+    intros.
+    destruct n. auto.
+    destruct i.
+    simpl in H. destruct (runGenHandler_ignore st (InputHandler i)). destruct p0.
+    simpl in H.
+    apply nth_error_In, in_app_or in H.
+    destruct H. apply out_of_model_no_recv in H. contradiction.
+    apply send_to_model_no_recv in H. contradiction.
+    simpl in H. destruct (runGenHandler_ignore st (RecvHandler r)). destruct p0.
+    simpl in H.
+    apply nth_error_In, in_app_or in H.
+    destruct H. apply out_of_model_no_recv in H. contradiction.
+    apply send_to_model_no_recv in H. contradiction.
+  Qed.
+
+  Lemma create_list_from_transition_nth_input :
+    forall st, forall i, forall n, forall p,
+      nth_error (snd (create_list_from_transition st i)) n = Some (Input p) -> n = 0.
+  Proof.
+    intros.
+    destruct n. auto.
+    destruct i.
+    simpl in H. destruct (runGenHandler_ignore st (InputHandler i)). destruct p0.
+    simpl in H.
+    apply nth_error_In, in_app_or in H.
+    destruct H. apply out_of_model_no_input in H. contradiction.
+    apply send_to_model_no_input in H. contradiction.
+    simpl in H. destruct (runGenHandler_ignore st (RecvHandler r)). destruct p0.
+    simpl in H.
+    apply nth_error_In, in_app_or in H.
+    destruct H. apply out_of_model_no_input in H. contradiction.
+    apply send_to_model_no_input in H. contradiction.
+  Qed.
+
+  Lemma create_list_from_transition_never_nil :
+    forall st st' : State, forall i : input_types,
+      create_list_from_transition st i <> (st', []).
+  Proof.
+    intros.
+    unfold create_list_from_transition.
+    induction i.
+    destruct (runGenHandler_ignore st (InputHandler a)). destruct p.
+    intro. apply pair_equal_spec in H. destruct H. inversion H0.
+    destruct (runGenHandler_ignore st (RecvHandler b)). destruct p.
+    intro. apply pair_equal_spec in H. destruct H. inversion H0.
+  Qed.
+
+  Lemma create_list_from_transition_never_null :
+    forall st : State, forall i : input_types,
+      length (snd (create_list_from_transition st i)) <> 0.
+  Proof.
+    intros.
+    intro. apply length_zero_iff_nil in H.
+    destruct (create_list_from_transition st i) eqn: Heq.
+    eapply create_list_from_transition_never_nil.
+    rewrite Heq. simpl in *. subst.
+    Unshelve. 2: apply s. auto.
+  Qed.
+
+  (*
+    We want to transform a list of input values in a sequence of
+  *)
+
+
+
+
+  (*
+    from a list of input values, it creates a sequence of actions representing the
+    actions of the protocol as follows :
+
+    val1 -> val2 -> val3 -> ...
+              |
+              |
+              |
+              v
+    Recv(val1) ++ output (exec Recvhandler on val1) ++ send (exec Recvhandler on val1) -> Input(val2) -> ...
+
+  The trick here is to represent only a prefix of the run long enough to be able to get after
+  a actual execution and do proof on it
+   *)
+  Fixpoint create_list_of_actions
+    (st : State)
+    (pr : PreRun)
+    (target : nat) : State * list SpecializedNodeModel :=
+    match target with
+    | 0 =>
+        create_list_from_transition st (pr 0)
+    | S target' =>
+        let (st', prefix) := create_list_of_actions st pr target' in
+        let (st'', res) := create_list_from_transition st' (pr target) in
+        (st'', prefix ++ res)
+    end.
+
+  Lemma create_list_of_action_longer_than_target :
+    forall st : State, forall pr : PreRun, forall target : nat,
+      length (snd (create_list_of_actions st pr target)) > target.
+  Proof.
+    intros.
+    induction target ; simpl.
+    - destruct (create_list_of_actions st pr 0).
+      destruct (create_list_from_transition st (pr 0)) eqn : Heq.
+      assert (l0 <> []). intro. subst.
+      apply create_list_from_transition_never_nil in Heq. auto.
+      assert (length l0 <> 0). intro.
+      apply length_zero_iff_nil in H0. contradiction. simpl.
+      lia.
+    - destruct (create_list_of_actions st pr target).
+      destruct (create_list_from_transition s (pr (S target))) eqn : Heq. simpl.
+      rewrite app_length.
+      assert (l0 <> []). intro. subst.
+      apply create_list_from_transition_never_nil in Heq. auto.
+      assert (length l0 <> 0). intro.
+      apply length_zero_iff_nil in H0. contradiction. simpl in *.
+      lia.
+  Qed.
+
+  Lemma create_list_of_action_never_nil :
+    forall st st' : State, forall pr : PreRun, forall target : nat,
+      create_list_of_actions st pr target <> (st', []).
+  Proof.
+    intros.
+    destruct target ; simpl.
+    - apply create_list_from_transition_never_nil.
+    - destruct (create_list_of_actions st pr target).
+      destruct (create_list_from_transition s (pr (S target))) eqn : Heq.
+      intro. apply pair_equal_spec in H. destruct H. subst.
+      apply app_eq_nil in H0. destruct H0. subst. apply create_list_from_transition_never_nil in Heq. auto.
+  Qed.
+
+  Lemma list_of_actions_is_revertable :
+    forall st : State, forall pr : PreRun, forall target : nat,
+    exists l', exists st', snd (create_list_of_actions st pr target) = l' ++ (snd (create_list_from_transition st' (pr target))).
+  Proof.
+    destruct target.
+    - simpl.
+      destruct (pr 0) ; simpl.
+      destruct (runGenHandler_ignore st (InputHandler i)) eqn: Heq. destruct p eqn: Heq0.
+      subst.
+      exists []. exists st. rewrite Heq. simpl. auto.
+      destruct (runGenHandler_ignore st (RecvHandler r)) eqn: Heq. destruct p eqn: Heq0.
+      subst.
+      exists []. exists st. rewrite Heq. simpl. auto.
+    - simpl.
+      destruct (create_list_of_actions st pr target).
+      destruct (create_list_from_transition s (pr (S target))) eqn: Heq.
+      exists l. exists s. rewrite Heq. simpl. auto.
+  Qed.
+
+  Lemma list_of_actions_is_revertable_exact :
+    forall st : State, forall pr : PreRun, forall target : nat,
+      snd (create_list_of_actions st pr (S target)) =
+        (snd (create_list_of_actions st pr target)) ++ (snd (create_list_from_transition (fst (create_list_of_actions st pr target)) (pr (S target)))).
+  Proof.
+    intros.
+    simpl. destruct (create_list_of_actions st pr target). simpl.
+    destruct (create_list_from_transition s (pr (S target))). simpl.
+    auto.
+  Qed.
+
+  Lemma list_of_actions_is_revertable_extended :
+    forall st : State, forall pr : PreRun, forall target : nat, forall j : nat,
+      let (_, l) := create_list_of_actions st pr target in
+      j <= target ->
+      exists l' l'', exists st', l = l' ++ (snd (create_list_from_transition st' (pr j))) ++ l''.
+  Proof.
+    intros st pr.
+    assert (
+        forall i : nat, forall target : nat, forall j : nat,
+          let (_, l) := create_list_of_actions st pr target in
+          j <= target -> target - j = i ->
+          exists l'' l', exists st', l = l' ++ (snd (create_list_from_transition st' (pr j))) ++ l''
+      ).
+    induction i.
+    - intros. destruct (create_list_of_actions st pr target) eqn: Heq.
+      intros. assert (target = j) by lia. subst.
+      exists []. edestruct list_of_actions_is_revertable.
+      destruct H1. exists x. exists x0. rewrite app_nil_r, <- H1, Heq. simpl. auto.
+    - intros. destruct (create_list_of_actions st pr target) eqn: Heq.
+      intros.
+      specialize IHi with (target - 1) j.
+      destruct (create_list_of_actions st pr (target - 1)) eqn: Heq0.
+      assert (j <= target - 1). lia. apply IHi in H1. clear IHi.
+      destruct H1. destruct H1. destruct H1. simpl in Heq0.
+      subst. destruct target. lia. simpl in Heq0. assert (tmp : target - 0 = target) by lia. rewrite tmp in Heq0. clear tmp.
+      simpl in Heq. rewrite Heq0 in Heq.
+      destruct (create_list_from_transition s0 (pr (S target))).
+      apply pair_equal_spec in Heq. destruct Heq.
+      exists (x ++ l0), x0. exists x1. rewrite <-H2.
+      repeat rewrite app_assoc. auto. lia.
+    - intros. specialize H with (target - j) target j. destruct (create_list_of_actions st pr target).
+      intros. destruct H. lia. auto. destruct H. exists x0, x. auto.
+  Qed.
+
+  (*
+    Extract the nth action from a run
+  *)
+  Definition get_action (pr : PreRun) (st : State) (i : nat) : option NodeAction :=
+    let (_, l) := create_list_of_actions st pr i in
+    nth_error l i.
+
+  Lemma get_action_is_never_error :
+    forall pr : PreRun, forall st : State, forall i : nat,
+      get_action pr st i <> None.
+  Proof.
+    destruct i.
+    - unfold get_action.
+      assert (length (snd (create_list_of_actions st pr 0)) > 0). apply create_list_of_action_longer_than_target.
+      destruct (create_list_of_actions st pr 0).
+      simpl in H.
+      apply nth_error_Some. apply H.
+    - unfold get_action.
+      assert (length (snd (create_list_of_actions st pr (S i))) > S i). apply create_list_of_action_longer_than_target.
+      destruct (create_list_of_actions st pr (S i)).
+      simpl in H.
+      apply nth_error_Some. apply H.
+  Qed.
+
+  Import Arith.
+
+  Hypothesis recv_dec :
+    forall p p' : RecvType, {p = p'}+{p <> p'}.
+
+  Lemma reverse_act :
+    forall (pr : PreRun), forall st : State,
+    forall i : nat, forall p,
+      (get_action pr st) i = Some p ->
+      exists j : nat, exists l l', exists st',
+        In p (snd (create_list_from_transition st' (pr j))) /\
+          snd (create_list_of_actions st pr i) = l ++ (snd (create_list_from_transition st' (pr j))) ++ l'.
+  Proof.
+    intros pr st.
+    assert (
+        forall i i', forall p,
+          nth_error (snd (create_list_of_actions st pr i)) i' = Some p ->
+          exists j : nat, exists l l', exists st',
+            In p (snd (create_list_from_transition st' (pr j))) /\ snd (create_list_of_actions st pr i) = l ++ (snd (create_list_from_transition st' (pr j))) ++ l'
+      ).
+    induction i.
+    - intros. simpl in H.
+      exists 0. simpl. destruct (pr 0) ; simpl in * ;
+        exists [], [] ; exists st ; repeat split.
+      + destruct (runGenHandler_ignore st (InputHandler i)). destruct p0.
+        apply nth_error_In in H. auto.
+      + destruct (runGenHandler_ignore st (InputHandler i)).
+        destruct p0. simpl in *.
+        rewrite app_nil_r. auto.
+      + destruct (runGenHandler_ignore st (RecvHandler r)). destruct p0.
+        apply nth_error_In in H. auto.
+      + destruct (runGenHandler_ignore st (RecvHandler r)).
+        destruct p0. simpl in *.
+        rewrite app_nil_r. auto.
+    - intros. simpl in *.
+      destruct (create_list_of_actions st pr i) eqn: Heq.
+      destruct (create_list_from_transition s (pr (S i))) eqn: Heq0.
+      simpl in H. apply nth_error_In, in_app_or in H. destruct H.
+      + apply In_nth_error in H. destruct H. simpl in *.
+        specialize IHi with x p. apply IHi in H. repeat destruct H.
+        exists x0, x1, (x2++l0), x3. split. apply H.
+        repeat rewrite app_assoc in *.
+        apply <-app_inv_tail_iff. apply H0.
+      + apply In_nth_error in H.
+        destruct H. simpl in *.
+        exists (S i), l, [], s. split.
+        eapply nth_error_In. rewrite Heq0. simpl. apply H.
+        simpl. apply app_inv_head_iff.
+        rewrite Heq0. simpl. rewrite app_nil_r. auto.
+    - intros. eapply H.
+      unfold get_action in H0.
+      destruct (create_list_of_actions st pr i).
+      simpl. apply H0.
+  Qed.
+
+  Lemma reverse_recv :
+    forall (pr : PreRun), forall st : State,
+    forall i : nat, forall p,
+      (get_action pr st) i = Some (Recv p) ->
+      exists j : nat,
+        pr j = backend p.
+  Proof.
+    intros.
+    edestruct reverse_act.
+    apply H.
+    exists x.
+    repeat destruct H0.
+    apply In_nth_error in H0.
+    destruct H0.
+    assert (x3 = 0). eapply create_list_from_transition_nth_recv. apply H0.
+    subst.
+    destruct (pr x) ; simpl in *.
+    destruct (runGenHandler_ignore x2 (InputHandler i0)). destruct p0. simpl in H0. inversion H0.
+    destruct (runGenHandler_ignore x2 (RecvHandler r)). destruct p0. simpl in H0. inversion H0. auto.
+  Qed.
+
+  Lemma reverse_send :
+    forall (pr : PreRun), forall st : State,
+    forall i : nat, forall p,
+      (get_action pr st) i = Some (Input p) ->
+      exists j : nat,
+        pr j = frontend p.
+  Proof.
+    intros.
+    edestruct reverse_act.
+    apply H.
+    exists x.
+    repeat destruct H0.
+    apply In_nth_error in H0.
+    destruct H0.
+    assert (x3 = 0). eapply create_list_from_transition_nth_input. apply H0.
+    subst.
+    destruct (pr x) ; simpl in *.
+    destruct (runGenHandler_ignore x2 (InputHandler i0)). destruct p0. simpl in H0. inversion H0. auto.
+    destruct (runGenHandler_ignore x2 (RecvHandler r)). destruct p0. simpl in H0. inversion H0.
+  Qed.
+
+End local_representation.
+
+(***************************************
+  Later work
+***************************************)
+
+(*)
+Record Model (n : nat) :=
+  mkModel {
+      Process : Type;
+      ModelSpec : Type;
+      TranslateNodeSpec : Specification NodeAction -> (NodeSet n -> Process);
+      Translate
+      TranslateNetworkSpec : forall n : nat, Specification (ModelAction n) -> ModelSpec;
+      Certificate : (NodeSet n -> Process) -> ModelSpec -> ModelSpec -> Prop;
+    }.*)
+
+(*)
+Record Model :=
+  mkModel {
+      Certify : Specification NodeAction -> Interface -> Interface -> Prop
+  }
+.*)
+
+  (*)
+Arguments Process {n}.
+Arguments ModelSpec {n}.
+Arguments TranslateNodeSpec {n}.
+Arguments TranslateNetworkSpec {n}.
+Arguments Certificate {n}.*)
+
+Module Type Protocol.
+  Parameter I O I' O' : Type.
+  Parameter Frontend : @Interface I O.
+  Parameter Backend : @Interface I' O'.
+  Parameter State : Type.
+  Parameter input_handler output_handler : Type.
+  Parameter Spec : Specification (@NodeAction I O I' O').
+  Parameter Consistency : Type.
+  (*Parameter Model : Model.
+  Parameter Certification : Model.(Certify) Spec Backend Frontend.*)
+  (*)
+    forall n : nat, let m := Model n in
+             m.(Certificate)
+                     (m.(TranslateNodeSpec) Spec)
+                     (m.(TranslateNetworkSpec) n (fun t => Backend n (ProjectTraceOnInterface backend t)))
+                     (m.(TranslateNetworkSpec) n (fun t => Frontend n (ProjectTraceOnInterface frontend t)))
+  .*)
+End Protocol.
+
+
+Inductive ActionClass :=
+  | Intern_act
+  | Output_act
+  | Input_act
+  | Unused_act
+.
+
+Record AIOA (ActionPool : Type) :=
+  mkAIOA {
+    Classifier : ActionPool -> ActionClass;
+    Spec : Specification ActionPool;
+    UnusedHyp :
+      forall t : Trace ActionPool,
+        Spec t -> InvarientTrace (fun a => Classifier a <> Unused_act) t
+  }
+.
+
+Arguments Spec {ActionPool}.
+Arguments Classifier {ActionPool}.
+
+(*)
+
+Definition AIOA_TranslateNodeSpec {I O I' O'} {n : nat} (s : Specification NodeAction) (p : NodeSet n) : AIOA (@ModelAction I O I' O' n).
+  refine (
+    mkAIOA
+      (ModelAction n)
+      (
+        fun a : ModelAction n =>
+          let (p', act) := a in
+          if eq_dec p p' then
+            match act with
+              | Output _ | Send _ => Output_act
+              | _ => Input_act
+            end
+          else Unused_act
+      )
+      (
+        fun t : Trace (ModelAction n) =>
+          (forall n, forall p', p <> p' -> forall act, t n <> Some (p', act)) /\
+          s (TransformTrace
+              (fun a : ModelAction n =>
+                  let (p', act) := a in
+                  if eq_dec p p' then
+                    Some act
+                  else
+                    None)
+              t
+            )
+      )
+    _).
+  intros.
+  unfold InvarientTrace. intros.
+  case_eq (t i) ; intros ; auto.
+  intros. destruct m. case (eq_dec p n0) ; intros ; subst.
+  case n1 ; intros ; case i0 ; intros ; discriminate.
+  destruct H. specialize H with i n0 n1. apply H in n2.
+  contradiction.
+Defined.
+
+Definition AIOA_from_backend_spec_to_AIOA {n : nat} (i : Interface) : AIOA (ModelAction n).
+  refine (
+      mkAIOA
+        (ModelAction n)
+        (
+          fun a : ModelAction n =>
+            let (_, act) := a in
+            match act with
+              | Send _ => Input_act
+              | Recv _ => Output_act
+              | _ => Unused_act
+            end
+        )
+        (
+          fun t : Trace (ModelAction n) =>
+            (forall n, forall p, forall a, t n <> Some (p, frontend a)) /\
+              (i n) (TransformTrace
+                (fun a : ModelAction n =>
+                  let (p, act) := a in
+                    match act with
+                      | backend ia => Some (p, ia)
+                      | _ => None
+                    end
+                )
+                t
+            )
+        )
+        _
+    ).
+  intros.
+  unfold InvarientTrace.
+  intro. case_eq (t i0) ; auto ; intros.
+  destruct m. case_eq n1 ; intros.
+  - destruct H. specialize H with i0 n0 i1.
+    subst. contradiction.
+  - case i1 ; intro ; discriminate.
+Defined.
+
+Definition Compose
+  {CompType : Type}
+  {ActionPool : Type}
+  (non_empty : CompType)
+  (f : CompType -> AIOA ActionPool)
+  (ActClassDecideable : forall c : ActionClass, forall a : ActionPool, {forall t : CompType, (f t).(Classifier) a <> c}+{exists t : CompType, (f t).(Classifier) a = c})
+  : AIOA ActionPool.
+  refine (
+      mkAIOA
+        ActionPool
+        (
+          fun a : ActionPool =>
+            match (ActClassDecideable Output_act a, ActClassDecideable Input_act a) with
+              | (right _, _) => Output_act
+              | (left _, right _) => Input_act
+              | _ => if (ActClassDecideable Intern_act a) then Unused_act else Intern_act
+            end
+        )
+        (
+          fun t : Trace (ActionPool) =>
+            forall c : CompType, (f c).(Spec) t
+        )
+        _
+    ).
+  intros. unfold InvarientTrace.
+  intro. case_eq (t i) ; auto ; intros.
+  case (ActClassDecideable Output_act a) ; try discriminate ; intros.
+  case (ActClassDecideable Input_act a) ; try discriminate ; intros.
+  case (ActClassDecideable Intern_act a) ; try discriminate ; intros.
+  assert (forall comp : CompType, InvarientTrace (fun a => Classifier (f comp) a <> Unused_act) t).
+  intro. apply (UnusedHyp ActionPool). apply H.
+  intro.
+  case_eq (Classifier (f non_empty) a); intros.
+  - eapply n1. apply H3.
+  - eapply n. apply H3.
+  - eapply n0. apply H3.
+  - unfold InvarientTrace in H1. specialize H1 with non_empty i. rewrite H0 in H1. eapply H1. apply H3.
+Defined.
+
+Inductive CompType (n : nat) :=
+  | Node : NodeSet n -> CompType n
+  | Network : CompType n.
+
+Arguments Node {n}.
+Arguments Network {n}.
+
+Definition f
+  {n : nat}
+  (net : AIOA (ModelAction n))
+  (nodes : NodeSet n -> AIOA (ModelAction n))
+  (comp : CompType n) :
+  AIOA (ModelAction n) :=
+  match comp with
+    | Network => net
+    | Node p => nodes p
+  end.
+
+Definition AIOA_from_spec
+  (n : nat)
+
+
+
+
+
+
+
+
+
+
+
+Definition Certificate :
+
+.
+*)
