src/framework/multidim_parray.v
@@ -1,0 +1,312 @@
+Require Import PArray List.
+Require Import Uint63 ZArith.
+Require Import Lia.
+Require Import Bool.
+
+Set Implicit Arguments.
+
+Import ListNotations.
+
+Open Scope Z_scope.
+
+Fixpoint size_Z (format : list int) :=
+    match format with
+      | [] => 0%Z
+      | h::[] => to_Z h
+      | h::t =>
+          (to_Z h * size_Z t)%Z
+    end.
+
+Fixpoint size (format : list int) :=
+    match format with
+      | [] => 0%uint63
+      | h::[] => h
+      | h::t =>
+          (h * size t)%uint63
+    end.
+
+Record MultiArray A :=
+  mkMultiArray {
+    format : list int;
+    data : array A;
+  }.
+
+Open Scope uint63_scope.
+
+Fixpoint build_index (format : list int) (index : list int) : option int :=
+    match format, index with
+      | [], [] => None
+      | hf::[], hi::[] =>
+          if hi <? hf then
+            Some hi
+          else
+            None
+      | hf::tf, hi::ti =>
+          if hi <? hf then
+            match build_index tf ti with
+            | None => None
+            | Some i =>
+                Some (hi + hf*i)
+            end
+          else
+            None
+      | _, _ => None
+    end.
+
+Fixpoint well_formated_rec (index : list int) (format : list int) :=
+    match index, format with
+      | [], [] => true
+      | hi::ti, hf::tf =>
+          (hi <? hf)%uint63 && well_formated_rec ti tf
+      | _, _ => false
+    end.
+
+Definition well_formated {A : Type} (index : list int) (arr : @MultiArray A) :=
+    well_formated_rec index arr.(format).
+
+Definition make_multiarray {A : Type} (format : list int) (a : A) :=
+    mkMultiArray
+      format
+      (make (size format) a).
+
+Definition set_val {A : Type} (a : A) (index : list int) (arr : @MultiArray A) :=
+  match build_index arr.(format A) index with
+    | None => arr
+    | Some i =>
+        mkMultiArray
+          arr.(format A)
+          arr.(data A).[ i <- a ]
+  end.
+
+Definition get_val {A : Type} (index : list int) (arr : @MultiArray A) :=
+  match build_index arr.(format A) index with
+    | None => None
+    | Some i =>
+          Some arr.(data A).[ i ]
+  end.
+
+Section MultiArray.
+  Import ListNotations.
+
+  Variable A : Type.
+
+  Open Scope uint63_scope.
+  Open Scope Z_scope.
+
+  Remark size_Z_pos :
+    forall fmt, 0 <= size_Z fmt.
+  Proof.
+    induction fmt.
+    - simpl. lia.
+    - simpl.
+      assert (0 <= to_Z a < wB). apply to_Z_bounded. destruct fmt. lia. lia.
+  Qed.
+
+  Remark size_Z_is_size_for_less_than_wB :
+    forall fmt,
+      size_Z fmt < wB ->
+      size_Z fmt = to_Z (size fmt).
+  Proof.
+    induction fmt.
+    - intro. simpl. rewrite to_Z_0. auto.
+    - intro. simpl in *.
+      assert (0 <= to_Z a < wB). apply to_Z_bounded.
+      assert (0 <= size_Z fmt). apply size_Z_pos.
+      destruct fmt. auto.
+      rewrite mul_spec.
+      case_eq (to_Z a =? 0) ; intro.
+      apply Z.eqb_eq in H2. rewrite Z.mod_small ; lia.
+      apply Z.eqb_neq in H2. rewrite <- IHfmt.
+      rewrite Z.mod_small. lia. lia. nia.
+  Qed.
+
+  Close Scope Z_scope.
+
+  Lemma build_index_return_when_same_length :
+    forall format0 index i,
+      build_index format0 index = Some i ->
+      length format0 = length index.
+  Proof.
+    induction format0.
+    - intros. simpl in H. simpl.
+      destruct index ; auto.
+      inversion H.
+    - induction index.
+      + intros. simpl in H. destruct format0 ; inversion H.
+      + intros.
+        simpl. assert (length format0 = length index).
+        simpl in H. destruct format0. destruct index.
+        simpl. auto.
+        destruct (a0 <? a). simpl in H ; inversion H.
+        inversion H.
+        destruct (a0 <? a).
+        destruct (build_index (i0 :: format0) index) eqn: Heq.
+        eapply IHformat0. apply Heq. inversion H. inversion H. auto.
+  Qed.
+
+  Open Scope Z_scope.
+
+  Variable arr : @MultiArray A.
+  Hypothesis arr_format_is_small : (size_Z arr.(format) < wB).
+  Hypothesis arr_is_well_formated : (PArray.length arr.(data) = size arr.(format)).
+
+  Definition fmt : list int := arr.(format).
+  Lemma fmt_is_small :
+    (size_Z fmt < wB).
+  Proof.
+    unfold fmt. auto.
+  Qed.
+
+  Lemma build_index_in_bound_if_well_formated :
+    forall index i,
+      build_index fmt index = Some i ->
+      (i <? size fmt)%uint63 = true.
+  Proof.
+    intro index.
+    assert (fmt_is_small : size_Z fmt < wB). apply fmt_is_small.
+    revert fmt_is_small.
+    revert index.
+    generalize fmt as format0.
+    induction format0, index ;
+      try (intros ; simpl in H ; try destruct format0 ; inversion H ; fail).
+    intros.
+    simpl in H.
+    destruct format0. destruct index.
+    {
+      destruct (i <? a)%uint63 eqn: Heq. inversion H. subst. simpl.
+      rewrite ltb_spec in *. auto. inversion H.
+    }
+    {
+      destruct (i <? a)%uint63.
+      simpl in H ; inversion H.
+      inversion H.
+    }
+    destruct (i <? a)%uint63 eqn: Hineq.
+    destruct (build_index (i1 :: format0) index) eqn: Heq.
+    assert (0 <= to_Z a < wB). apply to_Z_bounded.
+    assert (0 <= to_Z i < wB). apply to_Z_bounded.
+    assert (0 <= to_Z i1 < wB). apply to_Z_bounded.
+    assert (0 <= to_Z i2 < wB). apply to_Z_bounded.
+    assert (0 <= to_Z (size format0) < wB). apply to_Z_bounded.
+    assert (0 <= size_Z format0). apply size_Z_pos.
+    apply IHformat0 in Heq.
+    inversion H. subst. clear H. simpl.
+    simpl in Heq.
+    rewrite ltb_spec in *.
+    simpl in fmt_is_small0.
+    destruct format0. simpl in *.
+    repeat (
+      rewrite mul_spec in *
+      || rewrite add_spec in *
+      || rewrite Z.mod_small
+      || rewrite <-size_Z_is_size_for_less_than_wB) ; auto ; try nia.
+    rewrite mul_spec in Heq. rewrite Z.mod_small in Heq.
+    assert (0 < to_Z i1). nia.
+    assert (0 < to_Z a). lia.
+    assert (φ (i1) * size_Z (i0::format0) < wB). nia.
+    assert (size_Z (i0::format0) < wB). nia.
+    rewrite <-size_Z_is_size_for_less_than_wB in Heq ; auto.
+    repeat (
+      rewrite mul_spec in *
+      || rewrite add_spec in *
+      || rewrite Z.mod_small
+      || rewrite <-size_Z_is_size_for_less_than_wB) ; auto ; try nia.
+    assert (0 < to_Z a). lia.
+    split. lia.
+    rewrite <-size_Z_is_size_for_less_than_wB. nia.
+    case_eq (to_Z i1 =? 0) ; intro.
+    apply Z.eqb_eq in H6. rewrite H6 in Heq. simpl in Heq.
+    rewrite Zmod_0_l in Heq. lia.
+    apply Z.eqb_neq in H6.
+    assert (φ (i1) * size_Z (i0::format0) < wB). nia.
+    nia. simpl. simpl in fmt_is_small0. rewrite ltb_spec in Hineq. nia.
+    inversion H. inversion H.
+  Qed.
+
+  Remark well_formated_rec_then_correct_index :
+    forall format0,
+      size_Z format0 < wB ->
+    forall index,
+      0 < to_Z (size format0) ->
+      well_formated_rec index format0 = true ->
+      build_index format0 index <> None.
+  Proof.
+    intros format0 H index. revert H.
+    revert index.
+    revert format0.
+    induction format0, index ; simpl ; intros format0_is_small ; intros.
+    - rewrite to_Z_0 in H. lia.
+    - rewrite to_Z_0 in H. lia.
+    - simpl in H0. inversion H0.
+    - destruct format0. destruct index.
+      destruct (i <? a)%uint63 eqn: Heq. discriminate.
+      simpl in H0. inversion H0.
+      destruct (i <? a)%uint63 eqn: Hineq ;
+        simpl in H0 ;  inversion H0.
+      destruct (i <? a)%uint63 eqn: Hineq.
+      destruct (build_index (i0 :: format0) index) eqn: Heq. discriminate.
+      contradict Heq. rewrite ltb_spec in Hineq.
+      assert (0 <= to_Z i < wB). apply to_Z_bounded.
+      assert (0 <= to_Z a < wB). apply to_Z_bounded.
+      assert (0 <= to_Z (size (i0 :: format0)) < wB). apply to_Z_bounded.
+      assert (size_Z (i0 :: format0) < wB). nia.
+      assert (0 < to_Z a). nia.
+      apply IHformat0.
+      rewrite mul_spec in H. rewrite Z.mod_small in H.
+      nia. split. nia. rewrite size_Z_is_size_for_less_than_wB in format0_is_small.
+      lia. lia. rewrite mul_spec in H. rewrite Z.mod_small in H. lia.
+      split. lia. rewrite size_Z_is_size_for_less_than_wB in format0_is_small.
+      lia. auto. auto. simpl in H0. inversion H0.
+    Qed.
+
+  Remark well_formated_then_correct_index :
+    forall index,
+      0 < to_Z (size arr.(format)) ->
+      well_formated index arr = true ->
+      build_index arr.(format) index <> None.
+  Proof.
+    intros.
+    apply well_formated_rec_then_correct_index ; auto.
+  Qed.
+
+  Lemma get_set_same :
+    forall a index,
+      0 < size_Z arr.(format) ->
+      well_formated index arr = true ->
+      get_val index (set_val a index arr) = Some a.
+  Proof.
+    intros.
+    unfold get_val, set_val.
+    destruct (build_index (format arr) index) eqn: Heq.
+    simpl. rewrite Heq. rewrite get_set_same. auto.
+    rewrite arr_is_well_formated.
+    eapply build_index_in_bound_if_well_formated.
+    apply Heq.
+    contradict Heq. apply well_formated_then_correct_index ; auto.
+    rewrite size_Z_is_size_for_less_than_wB in H ; auto.
+  Qed.
+
+  Lemma get_make :
+    forall a index,
+      0 < size_Z arr.(format) ->
+      well_formated index arr = true ->
+      @get_val A index (make_multiarray fmt a) = Some a.
+  Proof.
+    intros.
+    unfold get_val, make_multiarray. simpl in *.
+    destruct (build_index fmt index) eqn: Heq.
+    rewrite get_make. auto.
+    contradict Heq. apply well_formated_then_correct_index ; auto.
+    rewrite size_Z_is_size_for_less_than_wB in H ; auto.
+  Qed.
+
+  Lemma make_is_correct_length :
+    forall a : A,
+      (size fmt <=? max_length)%uint63 = true ->
+      PArray.length (make_multiarray fmt a).(data) = size fmt.
+  Proof.
+    intros.
+    unfold make_multiarray.
+    simpl. rewrite length_make. rewrite H. auto.
+  Qed.
+End MultiArray.
