src/framework/serialization.v
@@ -1,0 +1,227 @@
+Require Import String Ascii HexString BinNums BinPos.
+Require Import List Arith.
+Import ListNotations.
+
+Definition serialize_prefix_nat (n : nat) (s : string) : string :=
+  String.concat "H" [(of_nat n); s].
+
+Notation "s $ m" := (serialize_prefix_nat s m) (at level 70).
+
+(* This function allows one to desarialize the concatenation of two strings *)
+Fixpoint cut_on_H (input : string) : string*string :=
+  match input with
+    | EmptyString => (EmptyString, EmptyString)
+    | String a m' =>
+        if Ascii.eqb a "H" then
+          (EmptyString, m')
+        else
+          let (prefix, residual) := cut_on_H m' in
+          (String a prefix, residual)
+  end.
+
+Lemma cut_on_H_cut_on_first_H :
+  forall s s' : string, index 0 "H" s = None -> cut_on_H (s ++ String "H" s') = (s, s').
+Proof.
+  induction s.
+  - intros.
+    simpl. auto.
+  - intros.
+    simpl.
+    assert ((a =? "H")%char = false).
+    eapply index_correct3 in H ; auto.
+    case_eq ((a =? "H")%char) ; auto ; intros.
+    apply Ascii.eqb_eq in H0. subst. simpl in H.
+    destruct s ; simpl in H ; contradiction. discriminate. rewrite H0.
+    rewrite IHs ; auto.
+    unfold index in H.
+    case_eq (prefix "H" (String a s)) ; intro ;
+    rewrite H1 in H. inversion H.
+    fold index in H. case_eq (index 0 "H" s) ; intros ; auto.
+    rewrite H2 in H. inversion H.
+Qed.
+
+Open Scope positive_scope.
+
+Lemma double_is_bit_shift :
+  forall n, n*2 = n~0.
+Proof.
+  induction n.
+  - simpl. rewrite IHn. auto.
+  - simpl. rewrite IHn. auto.
+  - simpl. auto.
+Qed.
+
+Lemma plus1_simpl_in_lt :
+  forall n m, n+1 <= m -> n <= m.
+Proof.
+  intros.
+  eapply Pos.add_le_mono in H.
+  Unshelve.
+  3: apply 1. 3: apply 1~0.
+  rewrite Pos.add_comm in H.
+  assert (n+1+1 = 2+n). rewrite Pos.add_comm.
+  assert (n+1 = 1+n). rewrite Pos.add_comm. auto.
+  rewrite H0. clear H0. apply Pos.add_assoc.
+  rewrite H0 in H. clear H0.
+  apply Pos.add_le_mono_l in H. auto.
+  hnf. intro. cbv in H0. inversion H0.
+Qed.
+
+Lemma times2_simpl_in_lt :
+   forall n m, n*2 <= m -> n <= m.
+Proof.
+  intros.
+  eapply Pos.mul_le_mono in H.
+  Unshelve.
+  3: apply 1. 3: apply 1~0.
+  rewrite Pos.mul_comm in H.
+  assert (n*2*1 = 2*n). rewrite Pos.mul_comm.
+  assert (n*2 = 2*n). apply Pos.mul_comm.
+  rewrite H0. clear H0. apply Pos.mul_assoc.
+  rewrite H0 in H. clear H0.
+  apply Pos.mul_le_mono_l in H. auto.
+  hnf. intro. cbv in H0. inversion H0.
+Qed.
+
+Lemma bit_shift_doesnt_affect_order :
+  forall n m, n~0 <= m~1 -> n <= m.
+Proof.
+  intros.
+  apply Pos.leb_le.
+  destruct (n <=? m) eqn: Heq ; auto.
+  apply Bool.not_true_iff_false in Heq.
+  assert (~n <= m). intro. apply Heq. apply Pos.leb_le. auto.
+  apply Pos.lt_nle in H0.
+  assert (1 <= 1 + n - m - 1).
+  apply Pos.le_1_l.
+  rewrite Pos.add_comm in H1.
+  rewrite <-Pos.sub_add_distr in H1 ; auto.
+  assert (1+(m+1) <= n + 1 - (m+1) + (m+1)).
+  apply Pos.add_le_mono_r. auto.
+  assert (n + 1 - (m+1)+(m+1) = n+1 + (m+1) - (m+1)).
+  rewrite Pos.add_comm. rewrite Pos.add_sub_assoc.
+  rewrite Pos.add_comm. auto.
+  apply Pos.add_lt_mono_r. auto.
+  rewrite H3 in H2. clear H3.
+  rewrite Pos.add_sub in H2.
+  clear H1. assert (2*(1+(m+1)) <= 2*(n+1)).
+  apply Pos.mul_le_mono_l. auto.
+  repeat rewrite Pos.mul_add_distr_l in H1.
+  assert (2*1 = 2). simpl. auto. rewrite H3 in H1. clear H3.
+  rewrite Pos.add_comm in H1. apply Pos.add_le_mono_r in H1.
+  assert (2*m + 1 < 2*n).
+  rewrite Pos.add_1_r. apply Pos.le_succ_l.
+  repeat rewrite <-Pos.add_1_r. rewrite <-Pos.add_assoc.
+  assert (1+1=2). simpl. auto.
+  rewrite H3. auto.
+  rewrite <-double_is_bit_shift in H.
+  assert (forall n, n~1 = n*2+1). intro.
+  rewrite double_is_bit_shift. simpl. auto.
+  rewrite H4 in H.
+  rewrite Pos.mul_comm in H.
+  apply Pos.lt_nle in H.
+  auto. rewrite Pos.mul_comm. auto.
+  apply Pos.add_lt_mono_r. auto.
+Qed.
+
+Lemma trailing0_disappear :
+  forall n m, n~0 <= m~0 -> n <= m.
+Proof.
+  intros.
+  rewrite <-double_is_bit_shift in H.
+  assert (m~0 = m*2).
+  rewrite <-double_is_bit_shift. auto.
+  rewrite H0 in H. clear H0.
+  apply Pos.mul_le_mono_r in H. auto.
+Qed.
+
+Lemma trailing1_disappear :
+  forall n m, n~1 <= m~0 -> n <= m.
+Proof.
+  intros.
+  rewrite <-double_is_bit_shift in H.
+  assert (forall n, n~1 = n*2+1). intro.
+  rewrite double_is_bit_shift. simpl. auto.
+  rewrite H0 in H.
+  apply plus1_simpl_in_lt in H.
+  apply Pos.mul_le_mono_r in H. auto.
+Qed.
+
+Lemma of_pos_no_H : forall n, forall s, index 0 "H" s = None -> index 0 "H" (Raw.of_pos n s) = None.
+Proof.
+  assert (
+      forall n n', (n' <= n)%positive -> forall s, index 0 "H" s = None -> index 0 "H" (Raw.of_pos n' s) = None
+    ).
+  induction n.
+  - intros.
+    assert (forall n, n~1 = n*2+1). intro.
+    rewrite double_is_bit_shift. simpl. auto.
+    assert (forall n, n~0 = n*2). intro. rewrite double_is_bit_shift. auto.
+    destruct n' ; try destruct n' ; try destruct n' ; try destruct n' ; simpl ;
+        try apply IHn ; try (
+    repeat match goal with
+      | H: _~0 <= _~1 |- _ => apply bit_shift_doesnt_affect_order in H
+      | H: _~0 <= _ |- _ => rewrite H2 in H
+      | H: _~1 <= _ |- _ => rewrite H1 in H
+      | H: _ <= _~1 |- _ => rewrite H1 in H
+      | H: _ + 1 <= _ + 1 |- _ => apply Pos.add_le_mono_r in H
+      | H: _ * 2 <= _ * 2 |- _ => apply Pos.mul_le_mono_r in H
+      | H: _ + 1 <= _ |- _ => apply plus1_simpl_in_lt in H
+      | H: _ * 2 <= _ |- _ => apply times2_simpl_in_lt in H
+      | _ => auto
+    end ; simpl ; rewrite H0 ; auto).
+  - intros.
+    assert (forall n, n~1 = n*2+1). intro.
+    rewrite double_is_bit_shift. simpl. auto.
+    assert (forall n, n~0 = n*2). intro. rewrite double_is_bit_shift. auto.
+     destruct n' ; try destruct n' ; try destruct n' ; try destruct n' ; simpl ;
+        try apply IHn ; try (
+    repeat match goal with
+      | H: _~0 <= _~1 |- _ => apply bit_shift_doesnt_affect_order in H
+      | H: _~0 <= _~0 |- _ => apply trailing0_disappear in H
+      | H: _~1 <= _~0 |- _ => apply trailing1_disappear in H
+      | H: _~0 <= _ |- _ => rewrite H2 in H
+      | H: _~1 <= _ |- _ => rewrite H1 in H
+      | H: _ <= _~1 |- _ => rewrite H1 in H
+      | H: _ + 1 <= _ + 1 |- _ => apply Pos.add_le_mono_r in H
+      | H: _ * 2 <= _ * 2 |- _ => apply Pos.mul_le_mono_r in H
+      | H: _ + 1 <= _ |- _ => apply plus1_simpl_in_lt in H
+      | H: _ * 2 <= _ |- _ => apply times2_simpl_in_lt in H
+      | _ => auto
+    end ; simpl ; rewrite H0 ; auto).
+  - intros.
+    destruct (Pos.eq_dec n' 1).
+    subst. simpl. rewrite H0. auto.
+    contradict n.
+    apply Pos.le_antisym.
+    auto. apply Pos.le_1_l.
+  - intros. eapply H.
+    apply Pos.le_refl.
+    auto.
+Qed.
+
+Lemma of_N_no_H : forall n, index 0 "H" (of_N n) = None.
+Proof.
+  intro. destruct n. auto. simpl.
+  rewrite of_pos_no_H ; auto.
+Qed.
+
+Lemma of_nat_no_H : forall n : nat, index 0 "H" (of_nat n) = None.
+Proof.
+  intro. unfold of_nat. rewrite of_N_no_H. auto.
+Qed.
+
+Definition deserialize_prefix_nat (s : string) : nat*string :=
+  let (n_enc, s') := cut_on_H s in
+  let n := to_nat n_enc in
+  (n, s').
+
+Lemma deserialize_serialize_prefix_nat :
+  forall n : nat, forall s : string, deserialize_prefix_nat (n$s) = (n, s).
+Proof.
+  intros.
+  unfold deserialize_prefix_nat, serialize_prefix_nat.
+  simpl. repeat rewrite cut_on_H_cut_on_first_H.
+  - rewrite to_nat_of_nat. auto.
+  - apply of_nat_no_H.
+Qed.
