src/framework/test.v
@@ -1,0 +1,1824 @@
+Require Import MSets.
+Require Import Arith String Ascii BinaryString Init.Byte PArray List ListSet.
+Require Import framework.monad.
+Require Import Lia.
+Require Import common.tactic.
+Require Import framework.framework.
+Require Import Bool.
+
+Module Buffer := Make String_as_OT.
+
+Definition Message := string.
+
+Parameter NodeCount : nat.
+Definition f : nat := NodeCount / 3.
+Definition Node := nat.
+Definition Round := nat.
+
+Definition InputAction : Type := (Round * Message)%type.
+
+Inductive PacketType : Type :=
+  | Init
+  | Echo
+  | Ready
+.
+
+Definition PartialPacket : Type :=
+  PacketType*Message*Round*Node.
+
+Open Scope list_scope.
+Open Scope string_scope.
+
+(* We delimit the round with the letter D *)
+Definition serialize_partialpacket (_p : PartialPacket) : Message :=
+  let '(p, m, r, src) := _p in
+  match p with
+    | Init => String.concat "H" ((of_nat r)::(of_nat src)::(String "I" m)::nil)
+    | Echo => String.concat "H" ((of_nat r)::(of_nat src)::(String "E" m)::nil)
+    | Ready => String.concat "H" ((of_nat r)::(of_nat src)::(String "R" m)::nil)
+  end.
+
+Definition serialize_packet (n : Node) (m : Message) : Message :=
+  String.concat "H" ((of_nat n)::m::nil).
+
+Fixpoint cut_on_H (input : string) : string*string :=
+  match input with
+    | EmptyString => (EmptyString, EmptyString)
+    | String a m' =>
+        if Ascii.eqb a "H" then
+          (EmptyString, m')
+        else
+          let (prefix, residual) := cut_on_H m' in
+          (String a prefix, residual)
+  end.
+
+Definition deserialize_packet (m : Message) : option (Node*Message) :=
+  let (src_enc, data) := cut_on_H m in
+  let src := to_nat src_enc in
+  if (src <? NodeCount)%nat then Some (src, data) else None.
+(*)
+Definition deserialize_packet (m : Message) : option (Node*Message).
+  destruct (cut_on_H m) as (dest, data) eqn: H.
+  case_eq (to_nat dest <? NodeCount)%nat ; intro.
+  apply PeanoNat.Nat.ltb_lt in H0.
+  apply (Some (Fin.of_nat_lt H0, data)).
+  apply None.
+Defined.
+
+Print deserialize_packet.*)
+
+Lemma cut_on_H_cut_on_first_H :
+  forall s s' : string, index 0 "H" s = None -> cut_on_H (s ++ String "H" s') = (s, s').
+Proof.
+  induction s.
+  - intros.
+    simpl. auto.
+  - intros.
+    simpl.
+    assert ((a =? "H")%char = false).
+    eapply index_correct3 in H ; auto.
+    case_eq ((a =? "H")%char) ; auto ; intros.
+    apply Ascii.eqb_eq in H0. subst. simpl in H.
+    destruct s ; simpl in H ; contradiction. discriminate. rewrite H0.
+    rewrite IHs ; auto.
+    unfold index in H.
+    case_eq (prefix "H" (String a s)) ; intro ;
+    rewrite H1 in H. inversion H.
+    fold index in H. case_eq (index 0 "H" s) ; intros ; auto.
+    rewrite H2 in H. inversion H.
+Qed.
+
+Lemma of_pos_no_H : forall n, forall s, index 0 "H" s = None -> index 0 "H" (Raw.of_pos n s) = None.
+Proof.
+  induction n.
+  - intros. simpl. apply IHn. simpl. rewrite H. auto.
+  - intros. simpl. apply IHn. simpl. rewrite H. auto.
+  - intros. simpl. rewrite H. auto.
+Qed.
+
+Lemma of_N_no_H : forall n, index 0 "H" (of_N n) = None.
+Proof.
+  intro. destruct n. auto. simpl.
+  rewrite of_pos_no_H ; auto.
+Qed.
+
+Lemma of_nat_no_H : forall r : Round, index 0 "H" (of_nat r) = None.
+Proof.
+  intro. unfold of_nat. rewrite of_N_no_H. auto.
+Qed.
+
+Definition deserialize_partialpacket (m : Message) : option PartialPacket :=
+  let (round_enc, tmp) := cut_on_H m in
+  let (src_enc, data) := cut_on_H tmp in
+  let round := to_nat round_enc in
+  let src := to_nat src_enc in
+  match data with
+    | String a m' =>
+        match a with
+          | "I"%char => Some (Init, m', round, src)
+          | "E"%char => Some (Echo, m', round, src)
+          | "R"%char => Some (Ready, m', round, src)
+          | _ => None
+        end
+    | _ => None
+  end.
+
+Lemma serialize_desirialize_partialpacket_id :
+  forall p, deserialize_partialpacket (serialize_partialpacket p) = Some p.
+Proof.
+  intros.
+  unfold deserialize_partialpacket, serialize_partialpacket.
+  destruct p. destruct p. destruct p.
+  case p ; simpl ; intros ; repeat rewrite cut_on_H_cut_on_first_H ;
+    (repeat rewrite to_nat_of_nat ; auto) || apply of_nat_no_H.
+Qed.
+
+Lemma serialize_partialpacket_inj :
+  forall p p', serialize_partialpacket p = serialize_partialpacket p' -> p = p'.
+Proof.
+  intros.
+  assert (Some p = Some p').
+  repeat rewrite <-serialize_desirialize_partialpacket_id.
+  rewrite H ; auto. inversion H0. auto.
+Qed.
+
+Lemma serialize_deserialize_packet_id :
+  forall p, forall m, p < NodeCount -> deserialize_packet (serialize_packet p m) = Some (p, m).
+Proof.
+  intros.
+  unfold deserialize_packet, serialize_packet.
+  simpl. rewrite cut_on_H_cut_on_first_H.
+  rewrite to_nat_of_nat.
+  case_eq (p <? NodeCount)%nat ; intros ; auto.
+  apply PeanoNat.Nat.ltb_ge in H0. lia.
+  apply of_nat_no_H.
+Qed.
+
+Lemma serialize_packet_inj :
+  forall p p', forall m m', p < NodeCount -> p' < NodeCount -> serialize_packet p m = serialize_packet p' m' -> p = p' /\ m = m'.
+Proof.
+  intros.
+  assert (Some (p, m) = Some (p', m')).
+  repeat rewrite <-serialize_deserialize_packet_id ; auto.
+  rewrite H1 ; auto. inversion H2. auto.
+Qed.
+
+Definition serialize_source_round (src : Node) (r : Round) :=
+  String.concat "H" ((of_nat src)::(of_nat r)::nil).
+
+Definition deserialize_source_round (m : Message) : option (Node*Round)%type :=
+  let (src_enc, r_enc) := cut_on_H m in
+  let src := to_nat src_enc in
+  let r := to_nat r_enc in
+  if (src <? NodeCount)%nat then Some (src, r) else None.
+
+Lemma serialize_deserialize_source_round_id :
+  forall src, forall r, src < NodeCount -> deserialize_source_round (serialize_source_round src r) = Some (src, r).
+Proof.
+  intros.
+  unfold serialize_source_round, deserialize_source_round.
+  simpl. rewrite cut_on_H_cut_on_first_H.
+  repeat rewrite to_nat_of_nat.
+  case_eq (src <? NodeCount)%nat ; intro ; auto.
+  apply PeanoNat.Nat.ltb_ge in H0. lia.
+  apply of_nat_no_H.
+Qed.
+
+Record CurrentStep : Type :=
+  mkCurrentStep {
+      (* source H round if the current pair is in step1,
+         in theory, this buffer should only contains values where the source is itself *)
+      step1 : Buffer.t ;
+      (* source H round if the current pair is in step2 *)
+      step2 : Buffer.t ;
+      (* source H round if the current pair is in step3 *)
+      step3 : Buffer.t ;
+      (* source H round if the current pair is done *)
+      delivered : Buffer.t ;
+    }.
+
+Record State : Type :=
+  mkState {
+      (* the total number of nodes in the model *)
+      node_count : Node ;
+      (* the id of the current node *)
+      id : Node ;
+      (* the buffer storing all the (pertinent) received messages, that is, messages with a pair (source, round) not in delivered buffer *)
+      input_buffer : Buffer.t ;
+      (* the list of buffers for the steps *)
+      steps : CurrentStep ;
+    }.
+
+Definition Handler := GenHandler (Node*Message) State (Node*Round*Message) unit.
+
+Fixpoint broadcast (m : Message) (n : Node) : Handler :=
+  match n with
+    | 0 => send (n, m)
+    | S n' => (broadcast m n') ;; send (n, m)
+  end.
+
+Lemma broadcast_length_is_n :
+  forall m, forall n, forall st,
+    length (snd (runGenHandler_ignore st (broadcast m n))) = n+1.
+Proof.
+  intros.
+  induction n.
+  - unfold broadcast. monad_unfold. simpl. auto.
+  - simpl. monad_unfold. destruct (broadcast m n st).
+    destruct p. destruct p. simpl in *.
+    rewrite app_length. rewrite IHn. simpl. lia.
+Qed.
+
+Lemma broadcast_output_only_same_type :
+  forall m : Message, forall n : Node, forall st,
+    forall n', {nth_error (snd (runGenHandler_ignore st (broadcast m n))) n' = Some (n', m)}+{nth_error (snd (runGenHandler_ignore st (broadcast m n))) n' = None}.
+Proof.
+  intros.
+  induction n.
+  - intros. unfold broadcast. monad_unfold.
+    simpl.
+    destruct n'. left. simpl. auto.
+    right. simpl. destruct n' ; auto.
+  - intros. simpl.
+    assert (length (snd (runGenHandler_ignore st (broadcast m n))) = n+1) by apply broadcast_length_is_n.
+    monad_unfold.
+    destruct (broadcast m n). destruct p. destruct p. simpl in *.
+    destruct IHn.
+    assert (n' < length l). apply nth_error_Some. rewrite e. discriminate.
+    left.
+    rewrite nth_error_app1 ; auto.
+    assert (n' >= length l). apply nth_error_None. auto.
+    case_eq (n' =? length l)%nat ; intro ; simpl_arith_bool. subst.
+    left. rewrite nth_error_app2. assert (tmp: length l - length l = 0) by lia. rewrite tmp. clear tmp.
+    simpl. simpl in H. rewrite H.
+    assert (S n = n + 1) by lia. rewrite H1. auto. auto.
+    right.
+    rewrite nth_error_app2 ; auto.
+    destruct (n' - length l) eqn: Heq. lia. simpl.
+    destruct n0 ; auto.
+Qed.
+
+Definition InputHandler (_m : Round*Message) : Handler :=
+  s <- get ;;
+  let (r, m) := _m in
+  if Buffer.mem (serialize_source_round s.(id) r) s.(steps).(delivered) ||
+      Buffer.mem (serialize_source_round s.(id) r) s.(steps).(step1) ||
+      Buffer.mem (serialize_source_round s.(id) r) s.(steps).(step2) ||
+      Buffer.mem (serialize_source_round s.(id) r) s.(steps).(step3) then
+    nop
+  else
+    let m := serialize_partialpacket (Init, m, r, s.(id)) in
+    broadcast m (NodeCount-1) ;;
+    put (
+        mkState
+          s.(node_count)
+          s.(id)
+          s.(input_buffer)
+          (mkCurrentStep
+             (Buffer.add (serialize_source_round s.(id) r) s.(steps).(step1))
+             s.(steps).(step2)
+             s.(steps).(step3)
+             s.(steps).(delivered)
+          )
+      )
+.
+
+Lemma input_handler_only_broadcast_init :
+  forall r : Round, forall m : Message, forall st,
+    forall n, {nth_error (snd (runGenHandler_ignore st (InputHandler (r, m)))) n =
+            Some (n, serialize_partialpacket (Init, m, r, st.(id)))} +
+           {nth_error (snd (runGenHandler_ignore st (InputHandler (r, m)))) n = None}.
+Proof.
+  intros.
+  unfold InputHandler. monad_unfold.
+  simpl.
+  destruct (Buffer.mem (serialize_source_round (id st) r) (delivered (steps st)) || Buffer.mem (serialize_source_round (id st) r) (step1 (steps st))
+       || Buffer.mem (serialize_source_round (id st) r) (step2 (steps st)) || Buffer.mem (serialize_source_round (id st) r) (step3 (steps st))).
+  intros. right. destruct n ; auto.
+  induction NodeCount.
+  - simpl. intros. destruct n. left. simpl. auto. right. simpl.
+    destruct n ; auto.
+  - assert (tmp : S n0 - 1 = n0) by lia. rewrite tmp. clear tmp.
+    destruct (broadcast (of_nat r ++ String "H" (of_nat (id st) ++ String "H" (String "I" m))) n0 st) eqn: Heq.
+    destruct p. destruct p. simpl in *.
+    edestruct broadcast_output_only_same_type with (of_nat r ++ String "H" (of_nat (id st) ++ String "H" (String "I" m))) n0 st n ;
+      monad_unfold ; rewrite Heq in e ; simpl in e.
+    left ; rewrite app_nil_r ; auto.
+    right ; rewrite app_nil_r ; auto.
+Qed.
+
+Definition filter_on_partial_packet (m : Message) (b : Buffer.t) :=
+  Buffer.filter (
+      fun m' =>
+        match deserialize_packet m' with
+          | None => false
+          | Some (src, data) =>
+              data =? m
+        end
+    ) b.
+
+Lemma filter_on_partial_packet_is_proper :
+  forall m : Message,
+    Proper (eq ==> eq)
+           (fun m' =>
+        match deserialize_packet m' with
+          | None => false
+          | Some (src, data) =>
+              data =? m
+        end
+    ).
+Proof.
+  intros. hnf. intros. subst. auto.
+Qed.
+
+Definition get_round_and_source_from_message (m : Message) : Round*Node :=
+  match deserialize_packet m with
+    | None => (0, 0)
+    | Some (src, data) =>
+        match deserialize_partialpacket data with
+          | None => (0, 0)
+          | Some (_, _, r, src) => (r, src)
+        end
+  end.
+
+Definition filter_except_round_and_source (r : Round) (src : Node) : Buffer.t -> Buffer.t :=
+  Buffer.filter (
+      fun m => let (r', src') := get_round_and_source_from_message m in
+            negb ((r' =? r)%nat && (src' =? src)%nat)
+    ).
+
+Lemma filter_on_round_is_proper :
+  forall r : Round, forall src : Node,
+    Proper (eq ==> eq)
+           (
+      fun m => let (r', src') := get_round_and_source_from_message m in
+            negb ((r' =? r)%nat && (src' =? src)%nat)
+    )
+.
+Proof.
+  intros. hnf. intros. subst. auto.
+Qed.
+
+Inductive Step :=
+  | NotStarted
+  | Step1
+  | Step2
+  | Step3
+  | Delivered
+.
+
+Definition Step_ltb (s s' : Step) : bool :=
+  match s, s' with
+    | NotStarted, NoStarted => false
+    | Step1, NotStarted | Step1, Step1 => false
+    | Step2, Step2 | Step2, Step1 | Step2, NotStarted => false
+    | Step3, Delivered => true
+    | Step3, _ => false
+    | Delivered, _ => false
+    | _, _ => true
+  end.
+
+Definition Step_lt (s s' : Step) : Prop :=
+  Step_ltb s s' = true.
+
+Notation "s << s'" := (Step_lt s s') (at level 70).
+
+Definition get_step (src : Node) (r : Round) (s : CurrentStep) : Step :=
+    let m := serialize_source_round src r in
+    if Buffer.mem m s.(delivered) then
+      Delivered
+    else if Buffer.mem m s.(step3) then
+      Step3
+    else if Buffer.mem m s.(step2) then
+      Step2
+    else if Buffer.mem m s.(step1) then
+      Step1
+    else
+      NotStarted.
+
+Definition increase_step (src : Node) (r : Round) (s : CurrentStep) : CurrentStep :=
+  match get_step src r s with
+    | NotStarted => s
+    | Delivered => s
+    | Step1 =>
+        mkCurrentStep
+          (Buffer.remove (serialize_source_round src r) s.(step1))
+          (Buffer.add (serialize_source_round src r) s.(step2))
+          s.(step3)
+          s.(delivered)
+    | Step2 =>
+        mkCurrentStep
+          s.(step1)
+          (Buffer.remove (serialize_source_round src r) s.(step2))
+          (Buffer.add (serialize_source_round src r) s.(step3))
+          s.(delivered)
+    | Step3 =>
+        mkCurrentStep
+          s.(step1)
+          s.(step2)
+          (Buffer.remove (serialize_source_round src r) s.(step3))
+          (Buffer.add (serialize_source_round src r) s.(delivered))
+  end
+.
+
+Lemma increase_step_equal_spec :
+  forall (src : Node) (r : Round) (s : CurrentStep),
+    match get_step src r s with
+      | NotStarted => get_step src r (increase_step src r s) = NotStarted
+      | Delivered => get_step src r (increase_step src r s) = Delivered
+      | Step1 => get_step src r (increase_step src r s) = Step2
+      | Step2 => get_step src r (increase_step src r s) = Step3
+      | Step3 => get_step src r (increase_step src r s) = Delivered
+    end.
+Proof.
+  intros.
+  unfold increase_step.
+  destruct (get_step src r s) eqn: Heq.
+  - auto.
+  - unfold get_step in *.
+    simpl in *.
+    destruct (Buffer.mem (serialize_source_round src r) (delivered s)). inversion Heq.
+    destruct (Buffer.mem (serialize_source_round src r) (step3 s)). inversion Heq.
+    assert (Buffer.mem (serialize_source_round src r) (Buffer.add (serialize_source_round src r) (step2 s)) = true).
+    apply Buffer.mem_spec. apply Buffer.add_spec. auto.
+    rewrite H. auto.
+  - unfold get_step in *.
+    simpl in *.
+    destruct (Buffer.mem (serialize_source_round src r) (delivered s)). inversion Heq.
+    assert (Buffer.mem (serialize_source_round src r) (Buffer.add (serialize_source_round src r) (step3 s)) = true).
+    apply Buffer.mem_spec. apply Buffer.add_spec. auto.
+    rewrite H. auto.
+  - unfold get_step in *.
+    simpl in *.
+    assert (Buffer.mem (serialize_source_round src r) (Buffer.add (serialize_source_round src r) (delivered s)) = true).
+    apply Buffer.mem_spec. apply Buffer.add_spec. auto.
+    rewrite H. auto.
+  - auto.
+Qed.
+
+Definition set_step (src : Node) (r : Round) (s : CurrentStep) (step : Step) :=
+  match step with
+    | NotStarted =>
+        mkCurrentStep
+          (Buffer.remove (serialize_source_round src r) s.(step1))
+          (Buffer.remove (serialize_source_round src r) s.(step2))
+          (Buffer.remove (serialize_source_round src r) s.(step3))
+          (Buffer.remove (serialize_source_round src r) s.(delivered))
+    | Delivered =>
+        mkCurrentStep
+          (Buffer.remove (serialize_source_round src r) s.(step1))
+          (Buffer.remove (serialize_source_round src r) s.(step2))
+          (Buffer.remove (serialize_source_round src r) s.(step3))
+          (Buffer.add (serialize_source_round src r) s.(delivered))
+    | Step1 =>
+        mkCurrentStep
+          (Buffer.add (serialize_source_round src r) s.(step1))
+          (Buffer.remove (serialize_source_round src r) s.(step2))
+          (Buffer.remove (serialize_source_round src r) s.(step3))
+          (Buffer.remove (serialize_source_round src r) s.(delivered))
+    | Step2 =>
+        mkCurrentStep
+          (Buffer.remove (serialize_source_round src r) s.(step1))
+          (Buffer.add (serialize_source_round src r) s.(step2))
+          (Buffer.remove (serialize_source_round src r) s.(step3))
+          (Buffer.remove (serialize_source_round src r) s.(delivered))
+    | Step3 =>
+        mkCurrentStep
+          (Buffer.remove (serialize_source_round src r) s.(step1))
+          (Buffer.remove (serialize_source_round src r) s.(step2))
+          (Buffer.add (serialize_source_round src r) s.(step3))
+          (Buffer.remove (serialize_source_round src r) s.(delivered))
+  end.
+
+Lemma set_step_equal_spec :
+  forall (src : Node) (r : Round) (s : CurrentStep),
+    forall step : Step,
+    get_step src r (set_step src r s step) = step.
+Proof.
+  intros.
+  unfold get_step, set_step.
+  destruct step ; simpl.
+  - assert (Buffer.mem (serialize_source_round src r) (Buffer.remove (serialize_source_round src r) (delivered s)) <> true).
+    intro. apply Buffer.mem_spec in H. apply Buffer.remove_spec in H. destruct H. contradiction.
+    destruct (Buffer.mem (serialize_source_round src r) (Buffer.remove (serialize_source_round src r) (delivered s))). contradiction.
+    assert (Buffer.mem (serialize_source_round src r) (Buffer.remove (serialize_source_round src r) (step3 s)) <> true).
+    intro tmp. apply Buffer.mem_spec in tmp. apply Buffer.remove_spec in tmp. destruct tmp. contradiction.
+    destruct (Buffer.mem (serialize_source_round src r) (Buffer.remove (serialize_source_round src r) (step3 s))). contradiction.
+    assert (Buffer.mem (serialize_source_round src r) (Buffer.remove (serialize_source_round src r) (step2 s)) <> true).
+    intro tmp. apply Buffer.mem_spec in tmp. apply Buffer.remove_spec in tmp. destruct tmp. contradiction.
+    destruct (Buffer.mem (serialize_source_round src r) (Buffer.remove (serialize_source_round src r) (step2 s))). contradiction.
+    assert (Buffer.mem (serialize_source_round src r) (Buffer.remove (serialize_source_round src r) (step1 s)) <> true).
+    intro tmp. apply Buffer.mem_spec in tmp. apply Buffer.remove_spec in tmp. destruct tmp. contradiction.
+    destruct (Buffer.mem (serialize_source_round src r) (Buffer.remove (serialize_source_round src r) (step1 s))). contradiction.
+    auto.
+  - assert (Buffer.mem (serialize_source_round src r) (Buffer.remove (serialize_source_round src r) (delivered s)) <> true).
+    intro. apply Buffer.mem_spec in H. apply Buffer.remove_spec in H. destruct H. contradiction.
+    destruct (Buffer.mem (serialize_source_round src r) (Buffer.remove (serialize_source_round src r) (delivered s))). contradiction.
+    assert (Buffer.mem (serialize_source_round src r) (Buffer.remove (serialize_source_round src r) (step3 s)) <> true).
+    intro tmp. apply Buffer.mem_spec in tmp. apply Buffer.remove_spec in tmp. destruct tmp. contradiction.
+    destruct (Buffer.mem (serialize_source_round src r) (Buffer.remove (serialize_source_round src r) (step3 s))). contradiction.
+    assert (Buffer.mem (serialize_source_round src r) (Buffer.remove (serialize_source_round src r) (step2 s)) <> true).
+    intro tmp. apply Buffer.mem_spec in tmp. apply Buffer.remove_spec in tmp. destruct tmp. contradiction.
+    destruct (Buffer.mem (serialize_source_round src r) (Buffer.remove (serialize_source_round src r) (step2 s))). contradiction.
+    assert (Buffer.mem (serialize_source_round src r) (Buffer.add (serialize_source_round src r) (step1 s)) = true).
+    apply Buffer.mem_spec. apply Buffer.add_spec. auto. rewrite H2. auto.
+  - assert (Buffer.mem (serialize_source_round src r) (Buffer.remove (serialize_source_round src r) (delivered s)) <> true).
+    intro. apply Buffer.mem_spec in H. apply Buffer.remove_spec in H. destruct H. contradiction.
+    destruct (Buffer.mem (serialize_source_round src r) (Buffer.remove (serialize_source_round src r) (delivered s))). contradiction.
+    assert (Buffer.mem (serialize_source_round src r) (Buffer.remove (serialize_source_round src r) (step3 s)) <> true).
+    intro tmp. apply Buffer.mem_spec in tmp. apply Buffer.remove_spec in tmp. destruct tmp. contradiction.
+    destruct (Buffer.mem (serialize_source_round src r) (Buffer.remove (serialize_source_round src r) (step3 s))). contradiction.
+    assert (Buffer.mem (serialize_source_round src r) (Buffer.add (serialize_source_round src r) (step2 s)) = true).
+    apply Buffer.mem_spec. apply Buffer.add_spec. auto. rewrite H1. auto.
+  - assert (Buffer.mem (serialize_source_round src r) (Buffer.remove (serialize_source_round src r) (delivered s)) <> true).
+    intro. apply Buffer.mem_spec in H. apply Buffer.remove_spec in H. destruct H. contradiction.
+    destruct (Buffer.mem (serialize_source_round src r) (Buffer.remove (serialize_source_round src r) (delivered s))). contradiction.
+    assert (Buffer.mem (serialize_source_round src r) (Buffer.add (serialize_source_round src r) (step3 s)) = true).
+    apply Buffer.mem_spec. apply Buffer.add_spec. auto. rewrite H0. auto.
+  - assert (Buffer.mem (serialize_source_round src r) (Buffer.add (serialize_source_round src r) (delivered s)) = true).
+    apply Buffer.mem_spec. apply Buffer.add_spec. auto. rewrite H. auto.
+Qed.
+
+Definition set_step_no_reset (src : Node) (r : Round) (s : CurrentStep) (step : Step) :=
+  match step with
+    | NotStarted => s
+    | Delivered =>
+        mkCurrentStep
+          s.(step1)
+          s.(step2)
+          s.(step3)
+          (Buffer.add (serialize_source_round src r) s.(delivered))
+    | Step1 =>
+        mkCurrentStep
+          (Buffer.add (serialize_source_round src r) s.(step1))
+          s.(step2)
+          s.(step3)
+          s.(delivered)
+    | Step2 =>
+        mkCurrentStep
+          s.(step1)
+          (Buffer.add (serialize_source_round src r) s.(step2))
+          s.(step3)
+          s.(delivered)
+    | Step3 =>
+        mkCurrentStep
+          s.(step1)
+          s.(step2)
+          (Buffer.add (serialize_source_round src r) s.(step3))
+          s.(delivered)
+  end.
+
+Definition set_step_no_reset_equal_spec :
+   forall (src : Node) (r : Round) (s : CurrentStep),
+    forall step : Step,
+    get_step src r s = NotStarted -> get_step src r (set_step_no_reset src r s step) = step.
+Proof.
+  intros.
+  unfold set_step_no_reset, get_step in *.
+  destruct step ; simpl in *.
+  - auto.
+  - destruct (Buffer.mem (serialize_source_round src r) (delivered s)).
+    inversion H.
+    destruct (Buffer.mem (serialize_source_round src r) (step3 s)).
+    inversion H.
+    destruct (Buffer.mem (serialize_source_round src r) (step2 s)).
+    inversion H.
+    assert (Buffer.mem (serialize_source_round src r) (Buffer.add (serialize_source_round src r) (step1 s)) = true).
+    apply Buffer.mem_spec. apply Buffer.add_spec. auto. rewrite H0. auto.
+  - destruct (Buffer.mem (serialize_source_round src r) (delivered s)).
+    inversion H.
+    destruct (Buffer.mem (serialize_source_round src r) (step3 s)).
+    inversion H.
+    assert (Buffer.mem (serialize_source_round src r) (Buffer.add (serialize_source_round src r) (step2 s)) = true).
+    apply Buffer.mem_spec. apply Buffer.add_spec. auto. rewrite H0. auto.
+  - destruct (Buffer.mem (serialize_source_round src r) (delivered s)).
+    inversion H.
+    assert (Buffer.mem (serialize_source_round src r) (Buffer.add (serialize_source_round src r) (step3 s)) = true).
+    apply Buffer.mem_spec. apply Buffer.add_spec. auto. rewrite H0. auto.
+  - assert (Buffer.mem (serialize_source_round src r) (Buffer.add (serialize_source_round src r) (delivered s)) = true).
+    apply Buffer.mem_spec. apply Buffer.add_spec. auto. rewrite H0. auto.
+Qed.
+
+Definition get_limit (step : Step) (p : PacketType) :=
+  match step with
+    | Step3 =>
+        match p with
+          | Ready => 2*f+1
+          | _ => 0
+        end
+    | _ =>
+        match p with
+          | Ready => f+1
+          | Echo => (NodeCount+f+1)/2
+          | _ => 0
+        end
+    end.
+
+Definition RecvHandler (_m : Node*Message) : Handler :=
+  s <- get ;;
+  let (src, m) := _m in
+  match deserialize_partialpacket m with
+    | None => nop
+    | Some (pm, data, r, proposer) =>
+  let step := get_step proposer r s.(steps) in
+  match step with
+    | Delivered => nop
+    | Step3 =>
+        match pm with
+          | Ready =>
+              let next_buffer := Buffer.add (serialize_packet src m) s.(input_buffer) in
+              if (Buffer.cardinal (filter_on_partial_packet m next_buffer) =? get_limit step pm)%nat then
+                write_output (proposer, r, data) ;;
+                put (
+                    mkState
+                      s.(node_count)
+                      s.(id)
+                      (
+                        filter_except_round_and_source r proposer s.(input_buffer)
+                      )
+                      (set_step proposer r s.(steps) Delivered)
+                  )
+              else
+                put (
+                    mkState
+                      s.(node_count)
+                      s.(id)
+                      next_buffer
+                      s.(steps)
+                  )
+            | _ => nop (* Either malformed or useless packet *)
+          end
+      | Step2 =>
+          match pm with
+            | Ready | Echo =>
+                let next_buffer := Buffer.add (serialize_packet src m) s.(input_buffer) in
+                (* check for the different conditions *)
+                if (Buffer.cardinal (filter_on_partial_packet m next_buffer) =? get_limit step pm )%nat then
+                  let m_to_send := serialize_partialpacket (Ready, data, r, proposer) in
+                  broadcast (m_to_send) (NodeCount-1) ;;
+                  put (
+                      mkState
+                        s.(node_count)
+                        s.(id)
+                        next_buffer
+                        (increase_step proposer r s.(steps))
+                  )
+                else
+                  put (
+                    mkState
+                      s.(node_count)
+                      s.(id)
+                      next_buffer
+                      s.(steps)
+                  )
+              | _ => nop
+            end
+        | Step1 | NotStarted =>
+            match pm with
+              | Init =>
+                  match step with
+                    | NotStarted =>
+                      let m_to_send := serialize_partialpacket (Echo, data, r, proposer) in
+                      broadcast m_to_send (NodeCount-1) ;;
+                      put (
+                          mkState
+                            s.(node_count)
+                            s.(id)
+                            s.(input_buffer)
+                            (set_step_no_reset proposer r s.(steps) Step2)
+                        )
+                      | _ => nop
+                    end
+              | Echo | Ready =>
+                  let next_buffer := Buffer.add (serialize_packet src m) s.(input_buffer) in
+                    (* check for the different conditions *)
+                    if (Buffer.cardinal (filter_on_partial_packet m next_buffer) =? get_limit step pm )%nat then
+                      (
+                        let m_to_send := serialize_partialpacket (Echo, data, r, proposer) in
+                        broadcast (m_to_send) (NodeCount-1)
+                      ) ;;
+                      let m_to_send := serialize_partialpacket (Ready, data, r, proposer) in
+                      broadcast (m_to_send) (NodeCount-1) ;;
+                      put (
+                          mkState
+                            s.(node_count)
+                            s.(id)
+                            next_buffer
+                            (set_step proposer r s.(steps) Step3)
+                      )
+                    else
+                      put (
+                        mkState
+                          s.(node_count)
+                          s.(id)
+                          next_buffer
+                          s.(steps)
+                      )
+            end
+        end end.
+
+Opaque serialize_partialpacket.
+
+Ltac autodestruct_broadcast :=
+  match goal with
+    | |- context [ broadcast ?a ?b ] =>
+        let H := fresh "Heq" in destruct (broadcast a b) eqn: H
+  end.
+
+Lemma recv_never_send_init :
+  forall n : Node, forall m : Message, forall st : State,
+    forall m', forall r, forall n', forall i j,
+      nth_error (snd (runGenHandler_ignore st (RecvHandler (n, m)))) i <> Some (j, serialize_partialpacket (Init, m', r, n')).
+Proof.
+  intros.
+  unfold RecvHandler. monad_unfold.
+  destruct (deserialize_partialpacket m) ; simpl ; cycle 1.
+  destruct i ; discriminate.
+  destruct p. destruct p. destruct p.
+  destruct (get_step n r0 (steps st)) ; simpl ;
+    try (destruct i ; discriminate) ; try destruct (_ =? _)%nat ; repeat (try autodestruct_broadcast ; repeat destruct p) ;
+  simpl ; try (destruct i ; discriminate) ; rewrite app_nil_r ;
+    (case_eq (i <? length l)%nat ; intro ; simpl_arith_bool ;
+     [ edestruct broadcast_output_only_same_type ;
+        monad_unfold ; try rewrite nth_error_app1 ; rewrite Heq in e |
+       edestruct broadcast_output_only_same_type ;
+        monad_unfold ; try rewrite nth_error_app2 ; rewrite Heq0 in e || rewrite Heq in e ] ;
+     auto) ; simpl in e ; try rewrite e ; try discriminate ; intro Hp ; inversion Hp as [H1] ;
+    apply serialize_partialpacket_inj in H0 ; inversion H0.
+Qed.
+
+Lemma buffer_monotone_before_delivering :
+  forall n : Node, forall m : Message, forall p : PacketType, forall r : Round, forall src : Node, forall st : State,
+    let '(_, st', _) := runGenHandler_ignore st (RecvHandler (n, serialize_partialpacket (p, m, r, src))) in
+    get_step n r st'.(steps) <> Delivered ->
+    Buffer.Subset (st.(input_buffer)) (st'.(input_buffer)).
+Proof.
+  intros.
+  unfold RecvHandler in *. monad_unfold.
+  rewrite serialize_desirialize_partialpacket_id.
+  destruct (get_step n r (steps st)) ; try destruct (_ =? _)%nat ;
+    repeat destruct p ; repeat (destruct (broadcast _ _ _) ; repeat destruct p) ;
+    unfold Buffer.Subset ; auto ; intros ; try apply Buffer.add_spec ; auto.
+  simpl in H.
+  unfold get_step in H. simpl in H.
+  assert (Buffer.mem (serialize_source_round n r)
+          (Buffer.add (serialize_source_round n r) (delivered (steps st))) = true).
+  apply Buffer.mem_spec. apply Buffer.add_spec. auto.
+  rewrite H1 in H. contradiction.
+Qed.
+
+Lemma recv_echo_acknowledge_before_step3 :
+  forall n : Node, forall m : Message, forall r : Round, forall src : Node, forall st : State,
+    let '(_, st', _) := runGenHandler_ignore st (RecvHandler (n, serialize_partialpacket (Echo, m, r, src))) in
+    get_step n r st'.(steps) << Step3 ->
+    Buffer.In (serialize_packet n (serialize_partialpacket (Echo, m, r, src))) st'.(input_buffer).
+Proof.
+  intros.
+  unfold RecvHandler, increase_step in *. monad_unfold.
+  rewrite serialize_desirialize_partialpacket_id.
+  destruct (get_step n r (steps st)) eqn: Heq ; try destruct (_ =? _)%nat ;
+    repeat destruct p ; repeat (destruct (broadcast _ _ _) ; repeat destruct p) ; auto ; intros ;
+    try apply Buffer.add_spec ; auto ; rewrite Heq in H ; hnf in H ; simpl in H ; inversion H.
+Qed.
+
+Opaque set_step.
+
+Lemma recv_ready_acknowledge_before_delivered :
+  forall n : Node, forall m : Message, forall r : Round, forall src : Node, forall st : State,
+    let '(_, st', _) := runGenHandler_ignore st (RecvHandler (n, serialize_partialpacket (Ready, m, r, src))) in
+    get_step n r st'.(steps) << Delivered ->
+    Buffer.In (serialize_packet n (serialize_partialpacket (Ready, m, r, src))) st'.(input_buffer).
+Proof.
+  intros.
+  unfold RecvHandler, increase_step in *. monad_unfold.
+  rewrite serialize_desirialize_partialpacket_id.
+  destruct (get_step n r (steps st)) eqn: Heq ; try destruct (_ =? _)%nat ;
+    repeat destruct p ; repeat (destruct (broadcast _ _ _) ; repeat destruct p) ; auto ; intros ;
+    try apply Buffer.add_spec ; auto ; simpl in * ; try rewrite set_step_equal_spec in H ; try rewrite Heq in H ;
+    hnf in H ; simpl in H ; inversion H.
+Qed.
+
+Require Import List.
+Import List.ListNotations.
+Open Scope list_scope.
+
+Require Import Permutation.
+Require Import PermutSetoid.
+Require Import Equalities.
+(*)
+Lemma dupA_then_dup :
+  forall A, forall l : list A, NoDupA eq l -> NoDup l.
+Proof.
+  intro A. induction l.
+  - intro. apply NoDup_nil.
+  - intro. inversion H.
+    apply NoDup_cons. intro. apply H2.
+    subst.
+    revert H4.
+    intro.
+    induction l.
+
+    intro. apply InA_nil. auto.
+    intro. apply InA_cons. subst.
+    right. apply IHl0. intro.
+  intros.
+  induction l
+
+  intros.
+  inversion H. subst. apply NoDup_nil.
+  apply NoDup_cons. intro. apply H0.
+  destruct l0. apply InA_nil. auto.
+
+  *)
+
+Lemma add_buffer_perm_buffer_add_element :
+  forall b : Buffer.t, forall m : Buffer.elt,
+    Buffer.mem m b <> true ->
+    length (Buffer.elements (Buffer.add m b)) = length (m::(Buffer.elements b)).
+Proof.
+  intros.
+  assert (permutation eq string_dec (Buffer.elements (Buffer.add m b)) (m::(Buffer.elements b))).
+  apply NoDupA_equivlistA_permut.
+  apply eq_equivalence.
+  apply Buffer.elements_spec2w.
+  apply NoDupA_cons.
+  intro. apply Buffer.elements_spec1 in H0.
+  apply H. apply Buffer.mem_spec. auto.
+  apply Buffer.elements_spec2w.
+  unfold equivlistA. intros. split ; intro.
+  apply Buffer.elements_spec1 in H0. apply Buffer.add_spec in H0.
+  destruct H0. subst. auto.
+  apply InA_cons. right. apply Buffer.elements_spec1. auto.
+  apply Buffer.elements_spec1. apply Buffer.add_spec.
+  apply InA_cons in H0. destruct H0 ; auto. apply Buffer.elements_spec1 in H0. auto.
+  apply permutation_Permutation in H0.
+  destruct H0.
+  destruct H0.
+  apply Forall2_length in H1. apply Permutation_length in H0.
+  rewrite H1 in H0. auto.
+  apply eq_equivalence.
+Qed.
+
+Lemma add_buffer_then_stricly_bigger :
+  forall b : Buffer.t, forall m : Buffer.elt,
+    Buffer.mem m b <> true ->
+    Buffer.cardinal (Buffer.add m b) = Buffer.cardinal b + 1.
+Proof.
+  intros.
+  apply add_buffer_perm_buffer_add_element in H.
+  simpl in H.
+  repeat rewrite Buffer.cardinal_spec. lia.
+Qed.
+
+Lemma add_buffer_perm_buffer :
+  forall b : Buffer.t, forall m : Buffer.elt,
+    Buffer.mem m b = true ->
+    length (Buffer.elements (Buffer.add m b)) = length (Buffer.elements b).
+Proof.
+  intros.
+  assert (permutation eq string_dec (Buffer.elements (Buffer.add m b)) (Buffer.elements b)).
+  apply NoDupA_equivlistA_permut.
+  apply eq_equivalence.
+  apply Buffer.elements_spec2w.
+  apply Buffer.elements_spec2w.
+  unfold equivlistA. intros. split ; intro.
+  apply Buffer.elements_spec1 in H0. apply Buffer.add_spec in H0.
+  destruct H0. subst. apply Buffer.mem_spec in H. apply Buffer.elements_spec1. auto.
+  apply Buffer.elements_spec1. auto. apply Buffer.elements_spec1.
+  apply Buffer.elements_spec1 in H0. apply Buffer.add_spec. auto.
+  apply permutation_Permutation in H0.
+  destruct H0.
+  destruct H0.
+  apply Forall2_length in H1. apply Permutation_length in H0.
+  rewrite H1 in H0. auto.
+  apply eq_equivalence.
+Qed.
+
+Lemma not_add_buffer_then_equal :
+  forall b : Buffer.t, forall m : Buffer.elt,
+    Buffer.mem m b = true ->
+    Buffer.cardinal (Buffer.add m b) = Buffer.cardinal b.
+Proof.
+  intros.
+  apply add_buffer_perm_buffer in H.
+  repeat rewrite Buffer.cardinal_spec. auto.
+Qed.
+
+Lemma add_increase_then_not_in_buffer_aux :
+  forall b : Buffer.t, forall m : Buffer.elt,
+    length (Buffer.elements (Buffer.add m b)) > length (Buffer.elements b)
+    -> Buffer.mem m b <> true.
+Proof.
+  intros.
+  assert (NoDupA eq (m :: Buffer.elements b)).
+  apply NoDupA_cons.
+  intro. apply Buffer.elements_spec1 in H0.
+  apply Buffer.mem_spec in H0. apply not_add_buffer_then_equal in H0.
+  repeat rewrite Buffer.cardinal_spec in H0. rewrite H0 in H. lia.
+  apply Buffer.elements_spec2w.
+  inversion H0. subst. intro. apply H3.
+  apply Buffer.elements_spec1. apply Buffer.mem_spec. auto.
+Qed.
+
+Lemma add_increase_then_not_in_buffer :
+  forall b : Buffer.t, forall m : Buffer.elt,
+    Buffer.cardinal (Buffer.add m b) > Buffer.cardinal b -> Buffer.mem m b <> true.
+Proof.
+  intros.
+  apply add_increase_then_not_in_buffer_aux.
+  repeat rewrite Buffer.cardinal_spec in H. auto.
+Qed.
+
+Lemma filter_add_either_add_or_not_m_not_m' :
+  forall n, n < NodeCount -> forall m m' : Message, forall b : Buffer.t,
+      m <> m' ->
+    Buffer.cardinal (filter_on_partial_packet m (Buffer.add (serialize_packet n m') b)) =
+      Buffer.cardinal (filter_on_partial_packet m b).
+Proof.
+  intros n H m m' b Heq.
+  repeat rewrite Buffer.cardinal_spec.
+   assert (
+       permutation eq string_dec
+                 (Buffer.elements (filter_on_partial_packet m (Buffer.add (serialize_packet n m') b)))
+                 (Buffer.elements (filter_on_partial_packet m b))
+     ).
+   apply NoDupA_equivlistA_permut.
+   apply eq_equivalence.
+   apply Buffer.elements_spec2w.
+   apply Buffer.elements_spec2w.
+   unfold equivlistA. intro. split ; intro.
+   + apply Buffer.elements_spec1 in H0. apply Buffer.elements_spec1.
+     apply Buffer.filter_spec in H0. apply Buffer.filter_spec.
+     apply filter_on_partial_packet_is_proper.
+     split. destruct H0.
+     apply Buffer.add_spec in H0. destruct H0. subst.
+     rewrite serialize_deserialize_packet_id in H1. apply String.eqb_eq in H1. subst ; contradiction.
+     auto. auto. apply H0. apply filter_on_partial_packet_is_proper.
+    + apply Buffer.elements_spec1. apply Buffer.elements_spec1 in H0.
+      apply Buffer.filter_spec in H0. apply Buffer.filter_spec.
+      apply filter_on_partial_packet_is_proper. destruct H0.
+      split ; auto. apply Buffer.add_spec. auto.
+      apply filter_on_partial_packet_is_proper.
+    + apply permutation_Permutation in H0. destruct H0.
+      destruct H0. apply Forall2_length in H1.
+      apply Permutation_length in H0.
+      rewrite H1 in H0. auto.
+      apply eq_equivalence.
+Qed.
+
+Lemma filter_add_either_add_or_not :
+  forall n, n < NodeCount -> forall m m' : Message, forall b : Buffer.t,
+    {Buffer.cardinal (filter_on_partial_packet m (Buffer.add (serialize_packet n m') b)) =
+      Buffer.cardinal (filter_on_partial_packet m b)}+{
+      Buffer.cardinal (filter_on_partial_packet m (Buffer.add (serialize_packet n m') b)) =
+      Buffer.cardinal (filter_on_partial_packet m b)+1
+    }.
+Proof.
+  intros.
+  destruct (string_dec m m').
+  - (* m = m' *)
+    subst m'.
+    destruct (Buffer.mem (serialize_packet n m) (filter_on_partial_packet m b)) eqn: Hmem.
+    {
+      left. apply Buffer.mem_spec, Buffer.filter_spec in Hmem.
+      repeat rewrite Buffer.cardinal_spec.
+      assert (permutation eq string_dec
+                (Buffer.elements (filter_on_partial_packet m (Buffer.add (serialize_packet n m) b)))
+                (Buffer.elements (filter_on_partial_packet m b))).
+      apply NoDupA_equivlistA_permut.
+      apply eq_equivalence.
+      apply Buffer.elements_spec2w.
+      apply Buffer.elements_spec2w.
+      unfold equivlistA. intro. split ; intro.
+      apply Buffer.elements_spec1.
+      apply Buffer.filter_spec. apply filter_on_partial_packet_is_proper.
+      apply Buffer.elements_spec1 in H0. apply Buffer.filter_spec in H0. destruct H0.
+      split. apply Buffer.add_spec in H0.
+      destruct H0. subst. apply Hmem. auto. auto.
+      apply filter_on_partial_packet_is_proper.
+      apply Buffer.elements_spec1 in H0. apply Buffer.elements_spec1.
+      apply Buffer.filter_spec in H0 ; try apply Buffer.filter_spec ; try apply filter_on_partial_packet_is_proper.
+      destruct H0. split. apply Buffer.add_spec. auto. auto.
+      apply permutation_Permutation in H0. destruct H0.
+      destruct H0. apply Forall2_length in H1.
+      apply Permutation_length in H0. rewrite H1 in H0. auto.
+      apply eq_equivalence. apply filter_on_partial_packet_is_proper.
+    }
+   {
+     right.
+     assert (
+         permutation eq string_dec
+                (Buffer.elements (filter_on_partial_packet m (Buffer.add (serialize_packet n m) b)))
+                ((serialize_packet n m)::(Buffer.elements (filter_on_partial_packet m b)))
+       ).
+     apply NoDupA_equivlistA_permut.
+     apply eq_equivalence.
+     apply Buffer.elements_spec2w.
+     apply NoDupA_cons. intro.
+     apply not_true_iff_false in Hmem. apply Hmem.
+     apply Buffer.mem_spec. apply Buffer.elements_spec1 in H0. auto.
+     apply Buffer.elements_spec2w.
+     unfold equivlistA. intro. split ; intro.
+     apply InA_cons. destruct (string_dec x (serialize_packet n m)) ; auto. right.
+     apply Buffer.elements_spec1.
+     apply Buffer.filter_spec. apply filter_on_partial_packet_is_proper.
+     apply Buffer.elements_spec1 in H0. apply Buffer.filter_spec in H0. destruct H0.
+     split. apply Buffer.add_spec in H0.
+     destruct H0. subst. contradiction. auto. auto.
+     apply filter_on_partial_packet_is_proper.
+     apply InA_cons in H0. destruct H0. subst.
+     apply Buffer.elements_spec1. apply Buffer.filter_spec. apply filter_on_partial_packet_is_proper.
+     split. apply Buffer.add_spec. auto. rewrite serialize_deserialize_packet_id. apply String.eqb_eq. auto. auto.
+     apply Buffer.elements_spec1 in H0. apply Buffer.elements_spec1.
+     apply Buffer.filter_spec in H0 ; try apply Buffer.filter_spec ; try apply filter_on_partial_packet_is_proper.
+     destruct H0. split. apply Buffer.add_spec. auto. auto.
+     apply permutation_Permutation in H0. destruct H0.
+     destruct H0. apply Forall2_length in H1.
+     apply Permutation_length in H0. rewrite H1 in H0. simpl in H0.
+     repeat rewrite Buffer.cardinal_spec.
+     assert (Datatypes.length (Buffer.elements (filter_on_partial_packet m b)) + 1 =
+               S (Datatypes.length (Buffer.elements (filter_on_partial_packet m b)))) by lia.
+     rewrite H2. auto.
+     apply eq_equivalence.
+   }
+ - (* m <> m' *)
+   eapply filter_add_either_add_or_not_m_not_m' in n0.
+   left. apply n0. auto.
+Qed.
+
+Lemma filter_add_either_add_or_not_m_not_m'_contrapose :
+  forall n, n < NodeCount -> forall m m' : Message, forall b : Buffer.t,
+  Buffer.cardinal (filter_on_partial_packet m (Buffer.add (serialize_packet n m') b)) =
+      Buffer.cardinal (filter_on_partial_packet m b) + 1 -> m = m'.
+Proof.
+  intros.
+  destruct (string_dec m m'). auto.
+  eapply filter_add_either_add_or_not_m_not_m' in n0. rewrite n0 in H0.
+  lia. auto.
+Qed.
+
+Lemma forall2_is_eq :
+  forall A, forall l l' : list A, Forall2 eq l l' -> l = l'.
+Proof.
+  intro. induction l.
+  - induction l'.
+    + auto.
+    + intro. inversion H.
+  - intros. inversion H. subst.
+    assert (l = l'0). apply IHl. auto. subst. auto.
+Qed.
+
+Lemma permutation_is_Permutation_with_eq :
+  forall l l', permutation eq string_dec l l' -> Permutation l l'.
+Proof.
+  intros.
+  apply permutation_Permutation in H ; try apply eq_equivalence.
+  destruct H. destruct H. apply forall2_is_eq in H0. subst. auto.
+Qed.
+
+Lemma recv_never_impact_other_pair :
+  forall n : Node, forall m : Message, forall r r' : Round, forall src src' : Node, forall p : PacketType, forall st : State,
+    let '(_, st', _) := runGenHandler_ignore st (RecvHandler (n, serialize_partialpacket (p, m, r, src))) in
+    Buffer.cardinal (filter_on_partial_packet (serialize_partialpacket (p, m, r', src')) st'.(input_buffer)) <>
+      Buffer.cardinal (filter_on_partial_packet (serialize_partialpacket (p, m, r', src')) st.(input_buffer)) ->
+    n < NodeCount ->
+    r = r' /\ src = src'.
+Proof.
+  intros.
+  unfold RecvHandler, increase_step in *. monad_unfold.
+  rewrite serialize_desirialize_partialpacket_id.
+  destruct (get_step n r (steps st)) eqn: Heq ; try destruct (_ =? _)%nat ;
+    repeat destruct p ; repeat (destruct (broadcast _ _ _) ; repeat destruct p) ; auto ; intros ;
+    try apply Buffer.add_spec ; auto ; simpl in * ; try lia ;
+    (edestruct filter_add_either_add_or_not ; try apply H0 ;
+    (rewrite e in H ; lia)
+    || (apply filter_add_either_add_or_not_m_not_m'_contrapose in e ; try apply serialize_partialpacket_inj in e ;
+    inversion e ; auto ; fail) ; fail)
+    || auto
+  .
+  repeat rewrite Buffer.cardinal_spec in H.
+  destruct ((r' =? r)%nat && (src =? src')%nat) eqn: Heqr. repeat simpl_arith_bool ; auto.
+  contradict H. apply Permutation_length.
+  assert (permutation eq string_dec
+         (Buffer.elements
+            (filter_on_partial_packet (serialize_partialpacket (Ready, m, r', src'))
+               (filter_except_round_and_source r src (input_buffer st))))
+         (Buffer.elements
+       (filter_on_partial_packet (serialize_partialpacket (Ready, m, r', src')) (input_buffer st)))).
+  apply NoDupA_equivlistA_permut.
+  apply eq_equivalence.
+  apply Buffer.elements_spec2w.
+  apply Buffer.elements_spec2w.
+  unfold equivlistA. intro. split ; intro.
+  - apply Buffer.elements_spec1. apply Buffer.elements_spec1 in H.
+    apply Buffer.filter_spec in H. destruct H. apply Buffer.filter_spec in H.
+    destruct H. apply Buffer.filter_spec. apply filter_on_partial_packet_is_proper.
+    split ; auto. apply filter_on_round_is_proper.
+    apply filter_on_partial_packet_is_proper.
+  - apply Buffer.elements_spec1. apply Buffer.elements_spec1 in H.
+    apply Buffer.filter_spec in H. apply Buffer.filter_spec.
+    apply filter_on_partial_packet_is_proper.
+    split. destruct H.
+    apply Buffer.filter_spec. apply filter_on_round_is_proper.
+    split. apply H. unfold get_round_and_source_from_message.
+    destruct (deserialize_packet x). destruct p. apply String.eqb_eq in H1.
+    subst. rewrite serialize_desirialize_partialpacket_id.
+    apply negb_true_iff.
+    apply andb_false_iff. repeat simpl_arith_bool. left. simpl_arith_bool. auto. right. simpl_arith_bool. auto.
+    inversion H1.
+    apply H. apply filter_on_partial_packet_is_proper.
+  - apply permutation_is_Permutation_with_eq in H. auto.
+Qed.
+
+Lemma send_ready_satisfies_condition :
+  forall n : Node, forall m : Message, forall r : Round, forall src : Node, forall p : PacketType, forall st : State,
+    let '(_, _, _snd) := runGenHandler_ignore st (RecvHandler (n, serialize_partialpacket (p, m, r, src))) in
+    let '(_, _, _snd') := runGenHandler_ignore st (broadacst (serialize_partialpacket (Ready, m, r, src)) NodeCount) in
+    _snd' = _snd ->
+    p = Echo /\ Buffer.cardinal (filter_on_partial_packet m next_buffer) = get_limit step p
+
+Definition empty_step :=
+  mkCurrentStep
+    Buffer.empty
+    Buffer.empty
+    Buffer.empty
+    Buffer.empty
+.
+
+Definition init_state (n : nat) :=
+  mkState
+    NodeCount
+    n
+    Buffer.empty
+    empty_step
+.
+
+(* Now that we have written the implementation of our protocol, we have to prove that it satifies some local prop *)
+
+Definition input_types := ((Round*Message)+(Node*Message))%type.
+
+Definition PreRun : Type := nat -> input_types.
+
+Definition compute_transition
+      (st : State)
+      (i : input_types) :=
+  match i with
+    | inl q =>
+        runGenHandler_ignore st (InputHandler q)
+    | inr q =>
+        runGenHandler_ignore st (RecvHandler q)
+  end.
+
+Require Import List.
+Import ListNotations.
+
+Definition SpecializedNodeModel := @NodeAction (Round*Message) (Node*Round*Message) (Node*Message) (Round*Message).
+
+Fixpoint out_to_model (out : list (Node*Round*Message)) : list SpecializedNodeModel :=
+  match out with
+    | [] => []
+    | a::b => (Output a)::(out_to_model b)
+  end.
+
+Fixpoint send_to_model snd : list SpecializedNodeModel :=
+  match snd with
+    | [] => []
+    | a::b => (Send a)::(send_to_model b)
+  end.
+
+Lemma out_of_model_no_recv :
+  forall out, forall p, ~In (Recv p) (out_to_model out).
+Proof.
+  induction out.
+  - intros. simpl. auto.
+  - intros. simpl. intro. destruct H. inversion H.
+    eapply IHout. apply H.
+Qed.
+
+Lemma send_to_model_no_recv :
+  forall out, forall p, ~In (Recv p) (send_to_model out).
+Proof.
+  induction out.
+  - intros. simpl. auto.
+  - intros. simpl. intro. destruct H. inversion H.
+    eapply IHout. apply H.
+Qed.
+
+Lemma out_of_model_no_input :
+  forall out, forall p, ~In (Input p) (out_to_model out).
+Proof.
+  induction out.
+  - intros. simpl. auto.
+  - intros. simpl. intro. destruct H. inversion H.
+    eapply IHout. apply H.
+Qed.
+
+Lemma send_to_model_no_input :
+  forall out, forall p, ~In (Input p) (send_to_model out).
+Proof.
+  induction out.
+  - intros. simpl. auto.
+  - intros. simpl. intro. destruct H. inversion H.
+    eapply IHout. apply H.
+Qed.
+
+
+Definition create_list_from_transition
+      (st : State)
+      (i : input_types) : State * list SpecializedNodeModel :=
+  match i with
+    | frontend q =>
+        let '(_out, st', _send) := runGenHandler_ignore st (InputHandler q) in
+        (st', (Input q)::(out_to_model _out) ++ (send_to_model _send))
+    | backend q =>
+        let '(_out, st', _send) := runGenHandler_ignore st (RecvHandler q) in
+        (st', (Recv q)::(out_to_model _out) ++ (send_to_model _send))
+  end.
+
+Lemma create_list_from_transition_nth_recv :
+  forall st, forall i, forall n, forall p,
+    nth_error (snd (create_list_from_transition st i)) n = Some (Recv p) -> n = 0.
+Proof.
+  intros.
+  destruct n. auto.
+  destruct i.
+  simpl in H. destruct (runGenHandler_ignore st (InputHandler p0)). destruct p1.
+  simpl in H.
+  apply nth_error_In, in_app_or in H.
+  destruct H. apply out_of_model_no_recv in H. contradiction.
+  apply send_to_model_no_recv in H. contradiction.
+  simpl in H. destruct (runGenHandler_ignore st (RecvHandler p0)). destruct p1.
+  simpl in H.
+  apply nth_error_In, in_app_or in H.
+  destruct H. apply out_of_model_no_recv in H. contradiction.
+  apply send_to_model_no_recv in H. contradiction.
+Qed.
+
+Lemma create_list_from_transition_nth_input :
+  forall st, forall i, forall n, forall p,
+    nth_error (snd (create_list_from_transition st i)) n = Some (Input p) -> n = 0.
+Proof.
+  intros.
+  destruct n. auto.
+  destruct i.
+  simpl in H. destruct (runGenHandler_ignore st (InputHandler p0)). destruct p1.
+  simpl in H.
+  apply nth_error_In, in_app_or in H.
+  destruct H. apply out_of_model_no_input in H. contradiction.
+  apply send_to_model_no_input in H. contradiction.
+  simpl in H. destruct (runGenHandler_ignore st (RecvHandler p0)). destruct p1.
+  simpl in H.
+  apply nth_error_In, in_app_or in H.
+  destruct H. apply out_of_model_no_input in H. contradiction.
+  apply send_to_model_no_input in H. contradiction.
+Qed.
+
+Lemma create_list_from_transition_never_nil :
+  forall st st' : State, forall i : input_types,
+    create_list_from_transition st i <> (st', []).
+Proof.
+  intros.
+  unfold create_list_from_transition.
+  induction i.
+  destruct (runGenHandler_ignore st (InputHandler a)). destruct p.
+  intro. apply pair_equal_spec in H. destruct H. inversion H0.
+  destruct (runGenHandler_ignore st (RecvHandler b)). destruct p.
+  intro. apply pair_equal_spec in H. destruct H. inversion H0.
+Qed.
+
+Lemma create_list_from_transition_never_null :
+  forall st : State, forall i : input_types,
+    length (snd (create_list_from_transition st i)) <> 0.
+Proof.
+  intros.
+  intro. apply length_zero_iff_nil in H.
+  destruct (create_list_from_transition st i) eqn: Heq.
+  eapply create_list_from_transition_never_nil.
+  rewrite Heq. simpl in *. subst.
+  Unshelve. 2: apply s. auto.
+Qed.
+
+Fixpoint create_list_of_actions
+      (st : State)
+      (pr : PreRun)
+      (target : nat) : State * list SpecializedNodeModel :=
+  match target with
+    | 0 =>
+        create_list_from_transition st (pr 0)
+    | S target' =>
+        let (st', prefix) := create_list_of_actions st pr target' in
+        let (st'', res) := create_list_from_transition st' (pr target) in
+        (st'', prefix ++ res)
+  end.
+
+Lemma create_list_of_action_longer_than_target :
+  forall st : State, forall pr : PreRun, forall target : nat,
+    length (snd (create_list_of_actions st pr target)) > target.
+Proof.
+  intros.
+  induction target ; simpl.
+  - destruct (create_list_of_actions st pr 0).
+    destruct (create_list_from_transition st (pr 0)) eqn : Heq.
+    assert (l0 <> []). intro. subst.
+    apply create_list_from_transition_never_nil in Heq. auto.
+    assert (length l0 <> 0). intro.
+    apply length_zero_iff_nil in H0. contradiction. simpl.
+    lia.
+  - destruct (create_list_of_actions st pr target).
+    destruct (create_list_from_transition s (pr (S target))) eqn : Heq. simpl.
+    rewrite app_length.
+    assert (l0 <> []). intro. subst.
+    apply create_list_from_transition_never_nil in Heq. auto.
+    assert (length l0 <> 0). intro.
+    apply length_zero_iff_nil in H0. contradiction. simpl in *.
+    lia.
+Qed.
+
+Lemma create_list_of_action_never_nil :
+  forall st st' : State, forall pr : PreRun, forall target : nat,
+    create_list_of_actions st pr target <> (st', []).
+Proof.
+  intros.
+  destruct target ; simpl.
+  - apply create_list_from_transition_never_nil.
+  - destruct (create_list_of_actions st pr target).
+    destruct (create_list_from_transition s (pr (S target))) eqn : Heq.
+    intro. apply pair_equal_spec in H. destruct H. subst.
+    apply app_eq_nil in H0. destruct H0. subst. apply create_list_from_transition_never_nil in Heq. auto.
+Qed.
+
+Lemma list_of_actions_is_revertable :
+  forall st : State, forall pr : PreRun, forall target : nat,
+    exists l', exists st', snd (create_list_of_actions st pr target) = l' ++ (snd (create_list_from_transition st' (pr target))).
+Proof.
+  destruct target.
+  - simpl.
+    destruct (pr 0) ; simpl.
+    destruct (runGenHandler_ignore st (InputHandler p)) eqn: Heq. destruct p0 eqn: Heq0.
+    subst.
+    exists []. exists st. rewrite Heq. simpl. auto.
+    destruct (runGenHandler_ignore st (RecvHandler p)) eqn: Heq. destruct p0 eqn: Heq0.
+    subst.
+    exists []. exists st. rewrite Heq. simpl. auto.
+  - simpl.
+    destruct (create_list_of_actions st pr target).
+    destruct (create_list_from_transition s (pr (S target))) eqn: Heq.
+    exists l. exists s. rewrite Heq. simpl. auto.
+Qed.
+
+Lemma list_of_actions_is_revertable_exact :
+  forall st : State, forall pr : PreRun, forall target : nat,
+    snd (create_list_of_actions st pr (S target)) =
+      (snd (create_list_of_actions st pr target)) ++ (snd (create_list_from_transition (fst (create_list_of_actions st pr target)) (pr (S target)))).
+Proof.
+  intros.
+  simpl. destruct (create_list_of_actions st pr target). simpl.
+  destruct (create_list_from_transition s (pr (S target))). simpl.
+  auto.
+Qed.
+
+Lemma list_of_actions_is_revertable_extended :
+  forall st : State, forall pr : PreRun, forall target : nat, forall j : nat,
+    let (_, l) := create_list_of_actions st pr target in
+    j <= target ->
+    exists l' l'', exists st', l = l' ++ (snd (create_list_from_transition st' (pr j))) ++ l''.
+Proof.
+  intros st pr.
+  assert (
+      forall i : nat, forall target : nat, forall j : nat,
+        let (_, l) := create_list_of_actions st pr target in
+        j <= target -> target - j = i ->
+        exists l'' l', exists st', l = l' ++ (snd (create_list_from_transition st' (pr j))) ++ l''
+    ).
+  induction i.
+  - intros. destruct (create_list_of_actions st pr target) eqn: Heq.
+    intros. assert (target = j) by lia. subst.
+    exists []. edestruct list_of_actions_is_revertable.
+    destruct H1. exists x. exists x0. rewrite app_nil_r, <- H1, Heq. simpl. auto.
+  - intros. destruct (create_list_of_actions st pr target) eqn: Heq.
+    intros. (*)
+    edestruct list_of_actions_is_revertable. rewrite Heq in H1. destruct H1.
+    simpl in H1. subst.*)
+    specialize IHi with (target - 1) j.
+    destruct (create_list_of_actions st pr (target - 1)) eqn: Heq0.
+    assert (j <= target - 1). lia. apply IHi in H1. clear IHi.
+    destruct H1. destruct H1. destruct H1. simpl in Heq0.
+    subst. destruct target. lia. simpl in Heq0. assert (tmp : target - 0 = target) by lia. rewrite tmp in Heq0. clear tmp.
+    simpl in Heq. rewrite Heq0 in Heq.
+    destruct (create_list_from_transition s0 (pr (S target))).
+    apply pair_equal_spec in Heq. destruct Heq.
+    exists (x ++ l0), x0. exists x1. rewrite <-H2.
+    repeat rewrite app_assoc. auto. lia.
+  - intros. specialize H with (target - j) target j. destruct (create_list_of_actions st pr target).
+    intros. destruct H. lia. auto. destruct H. exists x0, x. auto.
+Qed.
+
+
+Definition get_action (pr : PreRun) (st : State) (i : nat) : option NodeAction :=
+  let (_, l) := create_list_of_actions st pr i in
+  nth_error l i.
+
+Lemma get_action_is_never_error :
+  forall pr : PreRun, forall st : State, forall i : nat,
+    get_action pr st i <> None.
+Proof.
+  destruct i.
+  - unfold get_action.
+    assert (length (snd (create_list_of_actions st pr 0)) > 0). apply create_list_of_action_longer_than_target.
+    destruct (create_list_of_actions st pr 0).
+    simpl in H.
+    apply nth_error_Some. apply H.
+  - unfold get_action.
+    assert (length (snd (create_list_of_actions st pr (S i))) > S i). apply create_list_of_action_longer_than_target.
+    destruct (create_list_of_actions st pr (S i)).
+    simpl in H.
+    apply nth_error_Some. apply H.
+Qed.
+
+Require Import Arith.
+
+Lemma recv_dec :
+  forall p p' : Round*Message, {p = p'}+{p <> p'}.
+Proof.
+  intros.
+  destruct p, p'.
+  destruct PeanoNat.Nat.eq_dec with r r0. subst.
+  destruct string_dec with m m0. subst.
+  + left. auto.
+  + right. intro. apply pair_equal_spec in H. destruct H. contradiction.
+  + right. intro. apply pair_equal_spec in H. destruct H. contradiction.
+Qed.
+
+Lemma reverse_act :
+  forall (pr : PreRun), forall st : State,
+    forall i : nat, forall p,
+      (get_action pr st) i = Some p ->
+      exists j : nat, exists l l', exists st',
+        In p (snd (create_list_from_transition st' (pr j))) /\
+          snd (create_list_of_actions st pr i) = l ++ (snd (create_list_from_transition st' (pr j))) ++ l'.
+Proof.
+  intros pr st.
+  assert (
+      forall i i', forall p,
+        nth_error (snd (create_list_of_actions st pr i)) i' = Some p ->
+        exists j : nat, exists l l', exists st',
+        In p (snd (create_list_from_transition st' (pr j))) /\ snd (create_list_of_actions st pr i) = l ++ (snd (create_list_from_transition st' (pr j))) ++ l'
+    ).
+  induction i.
+  - intros. simpl in H.
+    exists 0. simpl. destruct (pr 0) ; simpl in * ;
+    exists [], [] ; exists st ; repeat split.
+    + destruct (runGenHandler_ignore st (InputHandler p0)). destruct p1.
+      apply nth_error_In in H. auto.
+    + destruct (runGenHandler_ignore st (InputHandler p0)).
+      destruct p1. simpl in *.
+      rewrite app_nil_r. auto.
+    + destruct (runGenHandler_ignore st (RecvHandler p0)). destruct p1.
+      apply nth_error_In in H. auto.
+    + destruct (runGenHandler_ignore st (RecvHandler p0)).
+      destruct p1. simpl in *.
+      rewrite app_nil_r. auto.
+  - intros. simpl in *.
+    destruct (create_list_of_actions st pr i) eqn: Heq.
+    destruct (create_list_from_transition s (pr (S i))) eqn: Heq0.
+    simpl in H. apply nth_error_In, in_app_or in H. destruct H.
+    + apply In_nth_error in H. destruct H. simpl in *.
+      specialize IHi with x p. apply IHi in H. repeat destruct H.
+      exists x0, x1, (x2++l0), x3. split. apply H.
+      repeat rewrite app_assoc in *.
+      apply <-app_inv_tail_iff. apply H0.
+    + apply In_nth_error in H.
+      destruct H. simpl in *.
+      exists (S i), l, [], s. split.
+      eapply nth_error_In. rewrite Heq0. simpl. apply H.
+      simpl. apply app_inv_head_iff.
+      rewrite Heq0. simpl. rewrite app_nil_r. auto.
+  - intros. eapply H.
+    unfold get_action in H0.
+    destruct (create_list_of_actions st pr i).
+    simpl. apply H0.
+Qed.
+
+Lemma reverse_recv :
+  forall (pr : PreRun), forall st : State,
+    forall i : nat, forall p,
+      (get_action pr st) i = Some (Recv p) ->
+      exists j : nat,
+        pr j = backend p.
+Proof.
+  intros.
+  edestruct reverse_act.
+  apply H.
+  exists x.
+  repeat destruct H0.
+  apply In_nth_error in H0.
+  destruct H0.
+  assert (x3 = 0). eapply create_list_from_transition_nth_recv. apply H0.
+  subst.
+  destruct (pr x) ; simpl in *.
+  destruct (runGenHandler_ignore x2 (InputHandler p0)). destruct p1. simpl in H0. inversion H0.
+  destruct (runGenHandler_ignore x2 (RecvHandler p0)). destruct p1. simpl in H0. inversion H0. auto.
+Qed.
+
+Lemma reverse_send :
+  forall (pr : PreRun), forall st : State,
+    forall i : nat, forall p,
+      (get_action pr st) i = Some (Input p) ->
+      exists j : nat,
+        pr j = frontend p.
+Proof.
+  intros.
+  edestruct reverse_act.
+  apply H.
+  exists x.
+  repeat destruct H0.
+  apply In_nth_error in H0.
+  destruct H0.
+  assert (x3 = 0). eapply create_list_from_transition_nth_input. apply H0.
+  subst.
+  destruct (pr x) ; simpl in *.
+  destruct (runGenHandler_ignore x2 (InputHandler p0)). destruct p1. simpl in H0. inversion H0. auto.
+  destruct (runGenHandler_ignore x2 (RecvHandler p0)). destruct p1. simpl in H0. inversion H0.
+Qed.
+
+Lemma ready_satisfies_cond :
+  forall pr : PreRun, forall n : Node,
+    n < NodeCount ->
+    forall i, forall p, forall m, forall r, get_action pr (init_state n) i = Some (Send (p, serialize_partialpacket (Ready m r))) ->
+
+                        BrachaRBStep (st BrachaRBAction (BrachaRBProcess f proc) (e i)) >= 3 /\ (
+                                 BrachaRBRecvBufferSize (st BrachaRBAction (BrachaRBProcess f proc) (e i)) (Echo m) >= 2*f+1 \/
+                                 BrachaRBRecvBufferSize (st BrachaRBAction (BrachaRBProcess f proc) (e i)) (Ready m) >= f+1
+                              )
+                   .
+Proof.
+  auto.
+Qed.
+
+
+
+
+Open Scope nat_scope.
+
+Fixpoint compute_action_aux (p : PreRun) (target : nat) (prerun_pointer : nat) (st : State) : option NodeAction :=
+  let (tmp, _send) := compute_transition st (p prerun_pointer) in
+  let (_out, st') := tmp in
+  match target with
+    | 0 =>
+        match (p prerun_pointer) with
+          | inl q => Some (Input q)
+          | inr q => Some (Recv q)
+        end
+    | S target' =>
+      if target' <? length _out then
+                  Some (Output (nth (target') _out (0, 0, "")))
+                else if target' - length _out <? length _send then
+                      Some (Send (nth (target' - length _out) _send (0, "")))
+                    else
+                      compute_action_aux p (target' - length _out - length _send) (prerun_pointer + 1) st'
+      end.
+
+Definition compute_action (p : PreRun) (st : State) : Trace NodeAction :=
+  fun n => compute_action_aux p n 0 st.
+
+Fixpoint compute_state_aux (p : PreRun) (st : State) (pos : nat) (steps : nat) : State :=
+  match steps with
+    | 0 => st
+    | S steps' =>
+        let (tmp, _) := compute_transition st (p pos) in
+        let (_, st') := tmp in
+        compute_state_aux p st' (pos+1) steps'
+  end.
+
+Definition compute_state (p : PreRun) (st : State) (steps : nat) : State :=
+  compute_state_aux p st 0 steps.
+
+Definition empty_step :=
+  mkCurrentStep
+    Buffer.empty
+    Buffer.empty
+    Buffer.empty
+    Buffer.empty
+.
+
+Definition init_state (n : nat) :=
+  mkState
+    NodeCount
+    n
+    Buffer.empty
+    empty_step
+.
+
+Definition Run (n : Node) (p : PreRun) := compute_action p (init_state n).
+
+Ltac unfold_run :=
+  unfold
+         Run,
+         compute_action,
+         compute_action_aux
+.
+(*)
+Lemma compute_transition_is_compute_state_unfold :
+  forall (n : Node) (pr : PreRun),
+    forall i,
+      compute_transition (compute_state pr (init_state n) i) (pr i) = compute_transition (compute_state pr (init_state n) (i+1)) (pr (i+1)).
+Proof.
+  intros.
+  induction i.
+  - unfold compute_transition, compute_state. simpl.*)
+
+(*)
+Lemma compute_action_is_compute_state :
+  forall (n : Node) (pr : PreRun),
+    forall i, forall inter,
+      Run n pr i = compute_action_aux pr i inter (compute_state pr (init_state n) inter).
+Proof.
+  intros n pr i.
+  induction i.
+  - intros. unfold_run. unfold compute_state, compute_state_aux.
+
+
+
+  induction inter.
+  - auto.
+  - rewrite IHinter. unfold compute_action_aux. destruct i.
+    destruct (compute_transition (compute_state pr (init_state n) inter) (pr inter)).
+    destruct p.
+    destruct (compute_transition (compute_state pr (init_state n) (S inter)) (pr (S inter))).
+    destruct p.
+    destruct (pr inter).
+    unfold Run, compute_action, compute_action_aux, compute_state, compute_state_aux in IHinter.
+    simpl in IHinter.
+
+    compute_transition (compute_state pr (init_state n) (S inter)) (pr (S inter)) = compute_transition (compute_state pr (init_state n) inter) (pr inter)
+
+
+    unfold compute_state, compute_state_aux. simpl.
+    destruct inter
+    destruct (compute_transition (compute_state pr (init_state n)))
+    unfold_run.
+    destruct i ; simpl.
+*)
+
+Ltac unfold_state :=
+  repeat unfold
+         compute_state,
+         compute_state_aux.
+
+Tactic Notation "unfold_run" "in" hyp(H) :=
+  repeat unfold
+         Run,
+         compute_action,
+         compute_action_aux
+  in H.
+
+Tactic Notation "unfold_transition" "in" hyp(H) :=
+  repeat unfold
+         compute_transition in H.
+
+Lemma reverse_recv :
+  forall (n : Node) (pr : PreRun),
+    let run := Run n pr in
+    forall i : nat, forall p,
+      run i = Some (Recv p) ->
+      exists j : nat,
+        pr j = backend p.
+Proof.
+  intros n pr run i. unfold run. clear run.
+  assert (forall k, k <= i -> forall p, Run n pr k = Some (Recv p) -> exists j, pr j = backend p).
+  induction i ; intros.
+  - assert (k = 0) by lia. subst. exists 0. unfold_run in H0.
+    destruct (compute_transition (init_state n) (pr 0)).
+    destruct p0.
+    destruct (pr 0) ; inversion H0. auto.
+  - destruct k. eapply IHi. 2: apply H0. lia.
+    unfold_run in H0.
+    fold compute_action_aux in H0. simpl in H0.
+    destruct (compute_transition (init_state n) (pr 0)).
+    destruct p0.
+    destruct (k <? length l0). inversion H0.
+    destruct (k - length l0 <? length l).
+    inversion H0.
+    eapply IHi ; cycle 1.
+    unfold_run.
+
+Lemma send_result_of_transition :
+  forall (n : Node) (pr : PreRun),
+    let run := Run n pr in
+    forall i : nat, forall p,
+      run i = Some (Output p) ->
+      exists j : nat,
+        let st := compute_state pr (init_state n) j in
+        let (tmp, _) := compute_transition st (pr j) in
+        let (_out, _) := tmp in
+        In p _out.
+Proof.
+  intros n pr run. unfold run in *. unfold Run, compute_action.
+  assert (forall i, forall k, forall p, forall inter, k <= i ->
+               compute_action_aux pr i inter (compute_state pr (init_state n) inter) = Some (Output p) ->
+               exists j : nat, let st := compute_state pr (init_state n) j in let (tmp, _) := compute_transition st (pr j) in let (_out, _) := tmp in In p _out
+         ).
+  induction i ; intros.
+  - unfold run in H0 ; unfold_run in H0. exists 0. simpl. unfold_state. assert (k = 0). lia. subst.
+    destruct (compute_transition (init_state n) (pr 0)). destruct p0. destruct (pr 0) ; inversion H0.
+  - destruct k. eapply IHi. 2: apply H0. lia.
+    unfold run in H0 ; unfold_run in H0. simpl in H0.
+    destruct (compute_transition (init_state n) (pr 0)) eqn: Htrans.
+    destruct p0 eqn: Hp0.
+    destruct (k <? length l0) eqn: Hlength. inversion H0. subst.
+    exists 0. simpl. unfold_state. rewrite Htrans.
+    apply nth_In. simpl_arith_bool. auto.
+    destruct (k - length l0 <? length l). inversion H0.
+    fold compute_action_aux in H0.
+
+
+
+
+    fold compute_action_aux in H, IHi. simpl in H
+
+
+    destruct (compute_state pr (init_state n) i).
+    simpl.
+
+
+
+
+  intros n pr run.
+  induction i.
+  - intros. exists 0. simpl.
+    destruct (compute_transition (compute_state pr (init_state n) 0) (pr 0)) eqn: Heq.
+    destruct p0 eqn : Heq0.
+    induction l0 ; intros ; unfold run in H ; unfold_run in H ; unfold compute_state in Heq ; simpl in Heq ;
+    rewrite Heq in H.
+    destruct (pr 0) ; inversion H.
+    destruct (pr 0) ; inversion H.
+  - intros.
+
+
+    
+    destruct (compute_state pr (init_state n) 0). simpl.
+    unfold run in H. unfold_run in H. simpl in H.
+    case_eq (pr 0) ; intros ; rewrite H0 in *.
+    destruct (runGenHandler_ignore (init_state n) (InputHandler p0)) in H.
+    destruct p1 in H. inversion H.
+    destruct (runGenHandler_ignore (init_state n) (RecvHandler p0)) in H.
+    destruct p1 in H. inversion H.
+  - intros. unfold run in H. unfold_run in H. simpl in H.
+    destruct (pr 0) eqn: Heq0.
+    destruct (runGenHandler_ignore (init_state n) (InputHandler p0)) eqn: Hrun.
+    destruct p1.
+    destruct (i <? length l0). inversion H.
+    destruct (i - length l0 <? length l). inversion H.
+
+
+
+
+
+  
+  forall run : Run,
+    forall p,
+    forall i : nat,
+      run.1 i = Some (Send p) ->
+      exists j : nat,
+        k
+
+Lemma echo_satisfies_cond :
+  forall ps : PreRun, forall n : Node,
+    n < NodeCount ->
+    let s := Run n ps in
+    forall i, forall p, forall m, s i = Some (Send (p, m)) -> True.
+Proof.
+  auto.
+Qed.
+
+
+
+
+
+
+
+
+
+
+
+Fixpoint compute_pos_and_offset_from_prerun (p : PreRun) (limit : nat) (prerun_pointer : nat) (st : State) :=
+  if limit =? 0 then
+    (prerun_pointer, 0)
+  else
+    match (p prerun_pointer) with
+      | left m =>
+          let () := runGenHandler_ignore st InputHandler
+      | right (n, m) =>.
+    let shift :=
+
+
+    compute_run_from_prerun_up_to_n p (
+        limit -
+
+      ) (prerun_pointer+1)
+
+Definition get_prerun_state_from_nat (p : PreRun) (n : nat) :=
+
+
+Definition run_from_prerun (p : PreRun) (n : nat) :
+$
