src/framework/test2.v
@@ -1,0 +1,420 @@
+Require Import Uint63.
+Require Import PArray List ListSet.
+Require Import monad.
+Require Import Lia.
+Require Import common.tactic.
+Require Import multidim_parray.
+
+Definition Message := list int.
+
+Lemma message_eq_dec :
+  forall m m' : Message, {m = m'}+{m <> m'}.
+Proof.
+  intros.
+  apply list_eq_dec.
+  intros.
+  case_eq (x =? y)%uint63 ; intro.
+  apply eqb_spec in H. auto.
+  assert ((x =? y) <> true). rewrite H. discriminate.
+  assert (x <> y). intro. apply H0.
+  apply eqb_spec. auto. auto.
+Qed.
+
+Parameter NodeCount : nat.
+Parameter f : nat.
+Parameter IdType : Type.
+Hypothesis eq_dec : forall p p' : IdType, {p = p'}+{p <> p'}.
+Definition Node := IdType.
+Definition Round := int.
+
+Parameter MaxRound : Round.
+
+Definition InputAction : Type := (Round * Message)%type.
+
+Inductive PacketType : Type :=
+  | Init
+  | Echo
+  | Ready
+.
+
+Definition PartialPacket : Type :=
+  PacketType*Round*Message.
+
+Local Open Scope uint63_scope.
+
+Record State :=
+  mkState {
+    id : IdType;
+    rounds : int;
+    process_ids : list IdType;
+    num_process : int;
+    message_recv : @MultiArray (option Message);
+    current_step : @MultiArray int;
+  }.
+
+Definition Handler := GenHandler (Node*Message) State (Node*Round*Message) unit.
+
+Import ListNotations.
+
+Fixpoint get_index_rec (pos : int) (id : IdType) (l : list IdType) :=
+  match l with
+    | [] => None
+    | h::t =>
+        if eq_dec h id then
+          Some pos
+        else
+          get_index_rec (pos+1) id t
+  end.
+
+Definition get_index (id : IdType) (s : State) :=
+  get_index_rec 0 id s.(process_ids).
+
+Definition get_message (r : Round) (t : PacketType) (_p : IdType) (s : State) :=
+  match get_index _p s with
+    | None => None
+    | Some p =>
+        let t_unpack := match t with
+                        | Init => 0
+                        | Echo => 0
+                        | Ready => 1
+                        end in
+        match get_val [r ; t_unpack ; p] s.(message_recv) with
+          | None => None
+          | Some a => a
+        end
+  end.
+
+Definition set_message (r : Round) (t : PacketType) (_p : IdType) (m : Message) (s : State) :=
+  match get_index _p s with
+    | None => s
+    | Some p =>
+        let t_unpack := match t with
+                        | Init => 0
+                        | Echo => 0
+                        | Ready => 1
+                        end in
+        mkState
+          s.(id)
+          s.(rounds)
+          s.(process_ids)
+          s.(num_process)
+          (set_val (Some m) [r ; t_unpack ; p] s.(message_recv))
+          s.(current_step)
+  end.
+
+Require Import ZArith.
+
+Section Message_handler.
+  Open Scope Z_scope.
+
+  Require Import Lra.
+
+  Variable state : State.
+  Hypothesis MaxRound_not_null : to_Z MaxRound > 0.
+  Hypothesis process_id_not_empty : to_Z state.(num_process) > 0.
+  Hypothesis num_process_is_process_ids_length :
+    to_Z state.(num_process) = Z.of_nat (length state.(process_ids)).
+  Hypothesis process_and_round_not_too_big :
+    size_Z (format (message_recv state)) < wB.
+  Hypothesis format_is_correct :
+    format (message_recv state) = [MaxRound ; 3%uint63 ; state.(num_process)].
+  Hypothesis array_is_of_size_format :
+    PArray.length (data (message_recv state)) = size (format (message_recv state)).
+
+  Remark to_Z_3 : to_Z 3 = 3.
+  Proof.
+    cbv. auto.
+  Qed.
+
+  Remark get_index_rec_invariant :
+    forall proc, forall i j : int, forall id : IdType,
+      get_index_rec i id proc = Some j ->
+      to_Z i + Z.of_nat (length proc) < wB ->
+      0 <= to_Z i ->
+      to_Z j < Z.of_nat (length proc) + to_Z i.
+  Proof.
+    induction proc.
+    - intros.
+      simpl in H. inversion H.
+    - intros. simpl in H. destruct (eq_dec a id0).
+      + inversion H. subst.
+        assert (length (id0::proc) = length proc+1)%nat. simpl. lia.
+        rewrite H2 in *. clear H2. lia.
+      + assert (length (a::proc) = length proc+1)%nat. simpl. lia.
+        rewrite H2 in *. clear H2.
+        apply IHproc in H. rewrite add_spec in H.
+        rewrite Nat2Z.inj_add in *. rewrite to_Z_1 in *. simpl in *.
+        rewrite Z.mod_small in H. lia.
+        assert (0 <= Z.of_nat (length proc)). apply Nat2Z.is_nonneg.
+        nia.
+        rewrite add_spec. rewrite Z.mod_small. rewrite to_Z_1. lia.
+        rewrite to_Z_1. nia.
+        rewrite add_spec. rewrite to_Z_1. rewrite Z.mod_small.
+        lia. nia.
+  Qed.
+
+  Remark get_index_limited_by_length :
+    forall id : IdType, forall i : int, get_index id state = Some i -> to_Z i < to_Z state.(num_process).
+  Proof.
+    intros.
+    unfold get_index in H.
+    apply get_index_rec_invariant in H.
+    rewrite to_Z_0 in H. rewrite num_process_is_process_ids_length. lia.
+    rewrite to_Z_0. simpl. rewrite <-num_process_is_process_ids_length.
+    assert (0 <= to_Z (num_process state) < wB). apply to_Z_bounded.
+    nia.
+    rewrite to_Z_0. lia.
+  Qed.
+
+  Remark get_index_rec_is_not_none_if_present :
+    forall l p i, In p l -> get_index_rec i p l <> None.
+  Proof.
+    induction l.
+    - simpl. auto.
+    - simpl. intros.
+      destruct H.
+      + subst.
+        destruct (eq_dec p p). discriminate.
+        contradiction.
+      + destruct (eq_dec a p). discriminate.
+        apply IHl. auto.
+  Qed.
+
+  Lemma get_set_message_same :
+    forall r : Round, forall t : PacketType, forall p : IdType, forall m : Message,
+      to_Z r < to_Z MaxRound ->
+      In p state.(process_ids) ->
+      get_message r t p (set_message r t p m state) = Some m.
+  Proof.
+    intros.
+    unfold get_message, set_message, get_index.
+    destruct (get_index_rec 0 p (process_ids state)) eqn: Heq.
+    simpl. rewrite Heq.
+    rewrite get_set_same ; auto.
+    rewrite format_is_correct.
+    assert (size_Z [MaxRound; 3%uint63; num_process state] =
+              (to_Z MaxRound) * (to_Z 3 * to_Z (num_process state))).
+    simpl. auto. rewrite H1. rewrite to_Z_3. nia.
+    unfold well_formated. simpl.
+    rewrite format_is_correct.
+    apply <-ltb_spec in H. rewrite H.
+    assert (to_Z i < to_Z (num_process state)).
+    eapply get_index_limited_by_length.
+    unfold get_index. apply Heq.
+    apply <-ltb_spec in H1. rewrite H1.
+    destruct t ; simpl ; auto.
+    contradict Heq. apply get_index_rec_is_not_none_if_present. auto.
+  Qed.
+End Message_handler.
+
+Definition get_step_index (r : Round) (p : int) (s : State) :=
+  match get_val [r ; p] s.(current_step) with
+    | None => 0
+    | Some q => q
+  end
+.
+
+Definition set_step_index (v : int) (r : Round) (p : int) (s : State) :=
+  mkState
+    s.(id)
+    s.(rounds)
+    s.(process_ids)
+    s.(num_process)
+    s.(message_recv)
+    (set_val v [r ; p] s.(current_step)).
+
+Definition get_step (r : Round) (_p : IdType) (s : State) :=
+  match get_index _p s with
+    | None => 0
+    | Some p =>
+        get_step_index r p s
+  end.
+
+Definition increase_step (r : Round) (_p : IdType) (s : State) :=
+  match get_index _p s with
+    | None => s
+    | Some p =>
+        set_step_index (get_step_index r p s + 1) r p s
+  end.
+
+Definition set_step (r : Round) (_p  : IdType) (step : int) (s : State) :=
+  match get_index _p s with
+    | None => s
+    | Some p =>
+        set_step_index step r p s
+  end.
+
+Section Step_handler.
+  Open Scope Z_scope.
+
+  Require Import Lra.
+
+  Variable state : State.
+  Hypothesis MaxRound_not_null : to_Z MaxRound > 0.
+  Hypothesis process_id_not_empty : to_Z state.(num_process) > 0.
+  Hypothesis num_process_is_process_ids_length :
+    to_Z state.(num_process) = Z.of_nat (length state.(process_ids)).
+  Hypothesis process_and_round_not_too_big :
+    size_Z (format (current_step state)) < wB.
+  Hypothesis format_is_correct :
+    format (current_step state) = [MaxRound ; state.(num_process)].
+  Hypothesis array_is_of_size_format :
+    PArray.length (data (current_step state)) = size (format (current_step state)).
+
+  Lemma get_set_step_index_same :
+    forall m r p,
+      to_Z r < to_Z MaxRound ->
+      to_Z p < to_Z state.(num_process) ->
+      get_step_index r p (set_step_index m r p state) = m.
+  Proof.
+    intros.
+    unfold get_step_index, set_step_index.
+    simpl.
+    rewrite get_set_same ; auto.
+    rewrite format_is_correct. simpl. nia.
+    unfold well_formated. simpl.
+    rewrite format_is_correct.
+    apply <-ltb_spec in H. apply <-ltb_spec in H0.
+    rewrite H, H0. simpl ; auto.
+  Qed.
+
+  Lemma get_set_step_same :
+    forall m r p,
+      to_Z r < to_Z MaxRound ->
+      In p state.(process_ids) ->
+      get_step r p (set_step r p m state) = m.
+  Proof.
+    intros.
+    unfold get_step, set_step, get_index.
+    destruct (get_index_rec 0 p (process_ids state)) eqn: Heq.
+    simpl. rewrite Heq.
+    rewrite get_set_step_index_same ; auto.
+    eapply get_index_limited_by_length ; auto.
+    unfold get_index. apply Heq.
+    contradict Heq. apply get_index_rec_is_not_none_if_present.
+    auto.
+  Qed.
+End Step_handler.
+
+Open Scope monad_scope.
+
+Fixpoint broadcast_rec (m : Message) (l : list IdType) (id : IdType) : Handler :=
+  match l with
+    | a::t =>
+        (if eq_dec a id then
+          send (a, m)
+        else
+          nop) ;; broadcast_rec m t id
+    | [] => nop
+  end
+.
+
+Definition broadcast (m : Message) (s : State) : Handler :=
+  broadcast_rec m s.(process_ids) s.(id).
+
+Definition serialize_packet (p : PartialPacket) :=
+  let '(t, r, m) := p in
+  match t with
+    | Init => 0::r::m
+    | Echo => 1::r::m
+    | Ready => 2::r::m
+  end
+.
+
+Definition deserialize_packet (_m : Message) :=
+  match _m with
+    | [] => None
+    | a::[] => None
+    | a::r::m =>
+        if a =? 0 then
+          Some (Init, r, m)
+        else if a =? 1 then
+          Some (Echo, r, m)
+        else if a =? 2 then
+          Some (Ready, r, m)
+        else None
+  end
+.
+
+Theorem deserialize_serialize_packet_is_id :
+  forall p, deserialize_packet (serialize_packet p) = Some p.
+Proof.
+  intros.
+  unfold deserialize_packet, serialize_packet.
+  destruct p. destruct p. destruct p ; auto.
+Qed.
+
+Definition InputHandler (_m : Round*Message) : Handler :=
+  s <- get ;;
+  let (round, m) := _m in
+  if get_step round s.(id) s =? 0 then
+    (* We didn't processed this round yet *)
+    (* broadcast to everyone but us *)
+    broadcast (serialize_packet (Init, round, m)) s ;;
+    (* Now, broadcast the echo and update our local view *)
+    broadcast (serialize_packet (Echo, round, m)) s ;;
+    put (set_step round s.(id) 1 (set_message round Echo s.(id) m s))
+  else nop
+.
+
+Definition process_init_packet
+  (n : Node)
+  (r : Round)
+  (m : Message)
+  (s : State) : Handler :=
+  if get_step r n s =? 0 then
+    (* We increase current step and set our own echo to m *)
+    put (set_message r Echo n m (set_step r n 1 s)) ;;
+    broadcast (serialize_packet (Echo, r, m)) s
+  else
+    (* This packet is invalid *)
+    nop
+.
+
+Definition acknowledge_recv
+  (n : Node)
+  (t : PacketType)
+  (r : Round)
+  (m : Message)
+  (s : State) : Handler :=
+  put (set_message r t n m s)
+.
+
+Fixpoint count_occurences_rec (r : Round) (pt : PacketType) (m : Message) (s : State) (l : list IdType) :=
+  match l with
+    | [] => 0
+    | h::t =>
+        match get_message r pt h s with
+          | None => count_occurences_rec r pt m s t
+          | Some m' =>
+              if message_eq_dec m' m then
+                1 + count_occurences_rec r pt m s t
+              else
+                count_occurences_rec r pt m s t
+        end
+  end
+.
+
+Definition count_occurences (r : Round) (pt : PacketType) (m : Message) (s : State) :=
+  count_occurences_rec r pt m s s.(process_ids).
+
+Definition RecvHandler (_m : Node*Message) : Handler :=
+  s <- get ;;
+  let (n, m_pack) := _m in
+  match deserialize_packet m_pack with
+    | None => nop
+    | Some (t, r, m) =>
+      match t with
+        | Init =>
+            process_init_packet n r m s
+        | Echo =>
+            acknowledge_recv n Echo r m s ;;
+            let st := get_step r n s in
+            (* we are interested in echos only in step 0 and 1 *)
+            if (st =? 0)%uint63 then
+              (* in this case, we broadcast an Echo as well as a Ready *)
+              (* we also have to update the step and the network view accordingly *)
+
+      end
+  end
+.
