src/framework/test3.v
@@ -1,0 +1,85 @@
+Require Import Arith.
+Require Import PArray List ListSet.
+Require Import monad.
+Require Import Lia.
+Require Import common.tactic.
+
+Definition Message := list nat.
+
+Parameter NodeCount : nat.
+Parameter f : nat.
+Parameter IdType : Type.
+Hypothesis eq_dec : forall p p' : IdType, {p = p'}+{p <> p'}.
+Definition Node := IdType.
+Definition Round := nat.
+
+Parameter MaxRound : Round.
+
+Definition InputAction : Type := (Round * Message)%type.
+
+Inductive PacketType : Type :=
+  | Init
+  | Echo
+  | Ready
+.
+
+Definition PartialPacket : Type :=
+  PacketType*Round*Message.
+
+Record State :=
+  mkState {
+    id : IdType;
+    rounds : nat;
+    process_ids : list IdType;
+    num_process : nat;
+    message_recv : array (option Message);
+    current_step : array nat;
+  }.
+
+Definition Handler := GenHandler (Node*Message) State (Node*Round*Message) unit.
+
+Import ListNotations.
+
+Fixpoint get_index_rec (pos : nat) (id : IdType) (l : list IdType) :=
+  match l with
+    | [] => None
+    | h::t =>
+        if eq_dec h id then
+          Some pos
+        else
+          get_index_rec (pos+1) id t
+  end.
+
+Definition get_index (id : IdType) (s : State) :=
+  get_index_rec 0 id s.(process_ids).
+
+Definition get_message (r : Round) (t : PacketType) (_p : IdType) (s : State) :=
+  match get_index _p s with
+    | None => None
+    | Some p =>
+        let t_unpack := match t with
+                        | Init => 0
+                        | Echo => 0
+                        | Ready => 1
+                        end in
+        s.(message_recv).[ (r * ( 3 * s.(num_process) ) + t_unpack * s.(num_process) + p) ]
+  end.
+
+Definition set_message (r : Round) (t : PacketType) (_p : IdType) (m : Message) (s : State) :=
+  match get_index _p s with
+    | None => s
+    | Some p =>
+        let t_unpack := match t with
+                        | Init => 0
+                        | Echo => 0
+                        | Ready => 1
+                        end in
+        mkState
+          s.(id)
+          s.(rounds)
+          s.(process_ids)
+          s.(num_process)
+
+          (PArray.set s.(message_recv) (r * ( 3 * s.(num_process) ) + t_unpack * s.(num_process) + p) (Some m))
+          s.(current_step)
+  end.
