src/ioa/ioa.v
@@ -1,0 +1,1423 @@
+Require Import List Arith Bool Lia Ensembles.
+Import ListNotations.
+
+Require Import common.tactic.
+
+(*)
+Possibly later used, but TO REMOVE
+
+Require Import Sets.Ensembles.
+Require Import RelationClasses.
+Require Import List.
+Require Import common.LTL.
+Require Import Nat.
+Require Import Arith.
+Require Import Bool.
+Require Import Classes.Equivalence.
+Require Import Relations.Relation_Definitions.
+Require Import common.tactic.
+Import ListNotations.
+Import Ensembles.
+Require Import Lia.*)
+
+
+
+(*
+  I want to use a variant of IOA.
+  If I simply transform them in
+  automaton, I can say that I
+  recognise the trace if :
+  1. Does not go to None state
+     This is automatic if we
+     don't put it as accepting
+     condition.
+  2. Does not stagned if an
+     action is enabled
+     This one is way more tricky
+     to specify, this is for
+     liveness
+     A solution might be to
+     identify a set of states
+     in which no internal or
+     output actions are enabled,
+     and set it a an acceptance
+     condition.
+
+ *)
+
+Record Signature (action_t : Type) : Type :=
+  mkSignature {
+      intern : Ensemble action_t;
+      output : Ensemble action_t;
+      input : Ensemble action_t;
+  }
+.
+
+Arguments intern {_} _.
+Arguments output {_} _.
+Arguments input {_} _.
+
+Definition ext
+  {action_t : Type}
+  (sig : Signature action_t)
+  : Ensemble action_t :=
+  Union
+    _
+    sig.(output)
+    sig.(input)
+.
+Definition acts
+  {action_t : Type}
+  (sig : Signature action_t)
+  : Ensemble action_t :=
+  Union
+    _
+    sig.(intern)
+    (ext sig)
+.
+Definition local
+  {action_t : Type}
+  (sig : Signature action_t)
+  : Ensemble action_t :=
+  Union
+    _
+    sig.(intern)
+    sig.(output)
+.
+Definition extsig
+  {action_t : Type}
+  (sig : Signature action_t)
+  : Signature action_t :=
+  mkSignature
+    _
+    (Empty_set _)
+    sig.(output)
+    sig.(input)
+.
+
+Definition sig_composition
+  {action_t : Type}
+  (sigA sigB : Signature action_t) :=
+  mkSignature
+    _
+    (Union _ sigA.(intern) sigB.(intern))
+    (Union _ sigA.(output) sigB.(output))
+    ( Setminus _ (Union _ sigA.(input) sigB.(input)) (Union _ sigA.(output) sigB.(output)))
+.
+
+Definition empty_sig
+  (action_t : Type)
+  : Signature action_t
+  :=
+  mkSignature
+    _
+    (Empty_set _)
+    (Empty_set _)
+    (Empty_set _)
+.
+
+Definition sig_hide
+  {action_t : Type}
+  (sig : Signature action_t)
+  (p : Ensemble action_t)
+  : Signature action_t :=
+  mkSignature
+    _
+    (Union _ sig.(intern) p)
+    (Setminus _ sig.(output) p)
+    (sig.(input))
+.
+
+Definition sig_dec
+  {action_t : Type}
+  (sig : Signature action_t) : Prop :=
+  forall a : action_t,
+    (In _ sig.(intern) a \/ ~In _ sig.(intern) a) /\
+      (In _ sig.(output) a \/ ~In _ sig.(output) a) /\
+      (In _ sig.(input) a \/ ~In _ sig.(input) a)
+.
+
+Definition
+  act_dec_t
+    {action_t : Type}
+    (sig : Signature action_t)
+    : Type :=
+  forall a : action_t,
+    {In _ (acts sig) a}+{~In _ (acts sig) a}
+.
+
+Global Hint Unfold ext acts local : sig.
+
+Section Signature.
+  Set Implicit Arguments.
+  Variable action_t : Type.
+
+  Variable sig : Signature action_t.
+
+  Ltac auto_solve_sig :=
+    unfold acts, ext, local in * ; auto with sets sig.
+
+  Lemma intern_in_act :
+    Included _ (intern sig) (acts sig).
+  Proof.
+    auto_solve_sig.
+  Qed.
+
+  Lemma output_in_act :
+    Included _ (output sig) (acts sig).
+  Proof.
+    auto_solve_sig.
+  Qed.
+
+  Lemma input_in_act :
+    Included _ (input sig) (acts sig).
+  Proof.
+    auto_solve_sig.
+  Qed.
+
+  Hint Resolve intern_in_act output_in_act input_in_act : sig.
+
+  Lemma local_in_act :
+    Included _ (local sig) (acts sig).
+  Proof.
+    auto_solve_sig.
+    unfold Included. intros. destruct H ; auto with sig.
+  Qed.
+
+  Lemma ext_in_act :
+    Included _ (ext sig) (acts sig).
+  Proof.
+    auto_solve_sig.
+  Qed.
+
+  Lemma intern_in_local :
+    Included _ (intern sig) (local sig).
+  Proof.
+    auto_solve_sig.
+  Qed.
+
+  Lemma output_in_local :
+    Included _ (output sig) (local sig).
+  Proof.
+    auto_solve_sig.
+  Qed.
+
+  Hint Resolve local_in_act ext_in_act intern_in_local output_in_local : sig.
+
+  Lemma act_to_local_input :
+    acts sig = Union _ (local sig) (input sig).
+  Proof.
+    apply Extensionality_Ensembles.
+    unfold Same_set. split.
+    - unfold Included. intros.
+      auto_solve_sig.
+      destruct H ; auto_solve_sig.
+      destruct H ; auto_solve_sig.
+    - unfold Included. intros.
+      auto_solve_sig.
+      destruct H ; auto_solve_sig.
+  Qed.
+
+  Lemma act_to_ext_intern :
+    acts sig = Union _ (ext sig) (intern sig).
+  Proof.
+    apply Extensionality_Ensembles.
+    unfold Same_set. split.
+    - unfold Included. intros.
+      auto_solve_sig.
+      destruct H ; auto_solve_sig.
+    - unfold Included. intros.
+      auto_solve_sig.
+      destruct H ; auto_solve_sig.
+  Qed.
+
+  Hint Rewrite act_to_local_input act_to_ext_intern : sig.
+
+  Lemma sig_act_dec :
+    forall a : action_t,
+      sig_dec sig ->
+      In _ (acts sig) a \/ ~In _ (acts sig) a.
+  Proof.
+    unfold sig_dec, acts.
+    intros.
+    specialize H with a.
+    destruct H as [Hi [HO HI]].
+    destruct Hi, HO, HI ; auto with sets sig.
+    right.
+    intro.
+    repeat destruct H2 ; auto with sets.
+  Qed.
+
+  Lemma union_commute :
+    forall T : Type,
+      forall a b : Ensemble T,
+        Union _ a b = Union _ b a.
+  Proof.
+    intros.
+    apply Extensionality_Ensembles.
+    unfold Same_set. split.
+    - unfold Included, In. intros.
+      destruct H.
+      apply Union_intror. auto.
+      apply Union_introl. auto.
+    - unfold Included, In. intros.
+      destruct H.
+      apply Union_intror. auto.
+      apply Union_introl. auto.
+  Qed.
+
+  Lemma union_dec :
+    forall T : Type,
+      forall a b : Ensemble T,
+        (forall t : T, In _ a t \/ ~In _ a t) ->
+        (forall t : T, In _ b t \/ ~In _ b t) ->
+        (forall t : T, In _ (Union _ a b) t \/ ~In _ (Union _ a b) t).
+  Proof.
+    intros.
+    edestruct H.
+    - left. unfold In. apply Union_introl. apply H1.
+    - edestruct H0. left. unfold In. apply Union_intror. apply H2.
+      right. intro. destruct H3 ; contradiction.
+  Qed.
+
+  Hint Resolve union_dec : sig.
+
+  Lemma setminus_dec :
+    forall T : Type,
+      forall a b : Ensemble T,
+        (forall t : T, In _ a t \/ ~In _ a t) ->
+        (forall t : T, In _ b t \/ ~In _ b t) ->
+        (forall t : T, In _ (Setminus _ a b) t \/ ~In _ (Setminus _ a b) t).
+  Proof.
+    intros.
+    edestruct H.
+    - edestruct H0. right. intro. unfold In, Setminus in H3.
+      destruct H3. apply H4. apply H2.
+      left. unfold In, Setminus. split ; auto. apply H1.
+    - right. intro. unfold In, Setminus in H2. destruct H2. contradiction.
+  Qed.
+
+  Hint Resolve setminus_dec : sig.
+
+  Variable sigA sigB : Signature action_t.
+
+  Lemma sig_composition_commute :
+    sig_composition sigA sigB = sig_composition sigB sigA.
+  Proof.
+    intros.
+    unfold sig_composition.
+    assert (Union action_t (intern sigA) (intern sigB) = Union action_t (intern sigB) (intern sigA)).
+    apply union_commute.
+    assert (Union action_t (output sigA) (output sigB) = Union action_t (output sigB) (output sigA)).
+    apply union_commute.
+    rewrite H. rewrite H0.
+    assert (Union action_t (input sigA) (input sigB) = Union action_t (input sigB) (input sigA)).
+    apply union_commute.
+    rewrite H1.
+    auto.
+  Qed.
+
+  Lemma included_local_act :
+    Included _ (local sigA) (acts sigA).
+  Proof.
+    unfold Included,
+           local,
+           acts,
+           In
+    .
+    intros.
+    destruct H.
+    - apply Union_introl. auto.
+    - apply Union_intror. unfold In. unfold ext. apply Union_introl.
+      auto.
+  Qed.
+
+  Hint Resolve included_local_act : sig.
+
+   Lemma sig_composition_keep_intern :
+    Included _ (intern sigA) (intern (sig_composition sigA sigB)).
+  Proof.
+    unfold Included, In, sig_composition.
+    intros. simpl.
+    apply Union_introl ; auto.
+  Qed.
+
+  Hint Resolve sig_composition_keep_intern : sig.
+
+  Lemma sig_composition_keep_output :
+    Included _ (output sigA) (output (sig_composition sigA sigB)).
+  Proof.
+    unfold Included, In, sig_composition.
+    intros. simpl.
+    apply Union_introl ; auto.
+  Qed.
+
+  Hint Resolve sig_composition_keep_output : sig.
+
+  Lemma sig_composition_keep_local :
+    Included _ (local sigA) (local (sig_composition sigA sigB)).
+  Proof.
+    unfold Included, local, In.
+    intros.
+    destruct H.
+    - apply Union_introl. auto with sig.
+    - apply Union_intror. apply Union_introl. auto with sig.
+  Qed.
+
+  Hint Resolve sig_composition_keep_local : sig.
+
+  Hypothesis HsigA_dec :
+    sig_dec sigA.
+  Hypothesis HsigB_dec :
+    sig_dec sigB.
+
+  Lemma sig_composition_keep_acts :
+    Included _ (acts sigA) (acts (sig_composition sigA sigB)).
+  Proof.
+    unfold Included, acts, In. intros.
+    destruct H.
+    - apply Union_introl.
+      auto with sig.
+    - apply Union_intror. unfold ext, In, sig_composition in *.
+      destruct H.
+      + apply Union_introl.
+        auto with sig.
+      + unfold sig_dec in *.
+        assert (In action_t (output sigA) x \/ ~ In action_t (output sigA) x).
+        apply HsigA_dec. destruct H0.
+        * apply Union_introl. unfold In. apply Union_introl. auto.
+        * assert (In action_t (output sigB) x \/ ~ In action_t (output sigB) x).
+          apply HsigB_dec. destruct H1.
+          apply Union_introl. unfold In. apply Union_intror. auto.
+          apply Union_intror. repeat unfold In, Setminus. split.
+          apply Union_introl. auto.
+          intro. destruct H2 ; contradiction.
+  Qed.
+
+  Hint Resolve sig_composition_keep_acts : sig.
+
+  Lemma sig_composition_dec :
+    sig_dec (sig_composition sigA sigB).
+  Proof.
+    unfold sig_dec. intro.
+    unfold sig_composition.
+    simpl.
+    repeat split.
+    - apply union_dec ; intro ; apply HsigA_dec || apply HsigB_dec.
+    - apply union_dec ; intro ; apply HsigA_dec || apply HsigB_dec.
+    - apply setminus_dec ; intro ; apply union_dec ; apply HsigA_dec || apply HsigB_dec.
+  Qed.
+
+  Hint Resolve sig_composition_dec : sig.
+
+  Lemma extsig_dec :
+    sig_dec (extsig sigA).
+  Proof.
+    unfold extsig, sig_dec.
+    intro.
+    repeat split ; simpl ; auto.
+    - right. unfold In. intro. destruct H.
+    - apply HsigA_dec.
+    - apply HsigA_dec.
+  Qed.
+
+  Hint Resolve extsig_dec : sig.
+
+  Unset Implicit Arguments.
+End Signature.
+
+Hint Rewrite act_to_local_input act_to_ext_intern : sig.
+
+Hint Resolve union_dec setminus_dec included_local_act sig_composition_keep_intern
+             sig_composition_keep_output sig_composition_keep_local sig_composition_keep_acts
+             sig_composition_dec extsig_dec local_in_act ext_in_act intern_in_local output_in_local
+  : sig.
+
+(*
+  We will create the IOA as a monad.
+  We create an invalid state, None,
+  which will be interpreted as an
+  invalid state. The reason for that
+  is to enforced a deterministic
+  behaviour of the system and making
+  it easier to specify some properties
+  like enabled actions.
+*)
+
+(*
+  Note : we need this strong assumption on sig for the
+  compositions lemma. If we only have decidability on the actions,
+  we cannot forward the lemma because of the way composition is built.
+ *)
+
+Record IOA (action_t : Type) : Type :=
+  mkIOA {
+      state_t : Type;
+      sig : Signature action_t;
+      initial : state_t -> Prop;
+      transition : state_t -> action_t -> option state_t;
+      act_dec : sig_dec sig;
+    }
+.
+
+Arguments state_t {_}.
+Arguments sig {_}.
+Arguments initial {_} _.
+Arguments transition {_} _ _.
+Arguments act_dec {_}.
+
+Section IOA.
+  Set Implicit Arguments.
+  Variable action_t : Type.
+
+  (* For now, we assume that every action that
+     is not in acts let the state unchange.
+     It is easier than assuming the decidbility
+     of sig I think
+   *)
+
+  Definition monad
+    (ioa : IOA action_t)
+    (s : option ioa.(state_t))
+    (a : action_t)
+    : option ioa.(state_t) :=
+    match s with
+      | None => None
+      | Some ss => ioa.(transition) ss a
+    end
+  .
+
+  Definition action_enabled
+    (ioa : IOA action_t)
+    (s : option ioa.(state_t))
+    (a : action_t)
+    : Prop :=
+    monad ioa s a <> None
+  .
+
+  (* We want to define a trace as finite because
+     traces will be executed and it is easier to
+     deal with liveness this way I think.
+     also because I really don't want to deal
+     with inductive types, too difficult for me *)
+  Definition trace_t (action_t : Type) : Type := list action_t.
+
+  Fixpoint execute_trace
+    (ioa : IOA action_t)
+    (s : option ioa.(state_t))
+    (t : trace_t action_t)
+    : option ioa.(state_t) :=
+    match t with
+      | [] => s
+      | h::t' => execute_trace ioa (monad ioa s h) t'
+    end
+  .
+
+  (*Notation "ioa >-> s t" := (execute_trace ioa s t) (at level 76, right associativity).*)
+
+
+  Notation "[ ioa ] s >-> t" := (execute_trace ioa s t) (at level 70).
+
+  Definition trace_enabled
+    (ioa : IOA action_t)
+    (s : option ioa.(state_t))
+    (t : trace_t action_t)
+    : Prop :=
+    [ioa] s >-> t <> None.
+
+  Lemma trace_not_enabled_on_none :
+    forall ioa : IOA action_t,
+    forall t : trace_t action_t,
+      ~ trace_enabled ioa None t.
+  Proof.
+    intro ioa.
+    induction t ; auto.
+  Qed.
+
+  Hint Resolve trace_not_enabled_on_none : ioa.
+
+  Definition trace_live
+    (ioa : IOA action_t)
+    (s : option ioa.(state_t))
+    (t : trace_t action_t)
+    : Prop :=
+    forall a : action_t,
+      In _ (local ioa.(sig)) a ->
+      ~ (action_enabled ioa ([ioa] s >-> t) a)
+  .
+
+  (*
+    A correct trace is a trace that is live
+    and enabled.
+   *)
+  Definition trace_correct
+    (ioa : IOA action_t)
+    (s : option ioa.(state_t))
+    (t : trace_t action_t)
+    : Prop :=
+    trace_enabled ioa s t /\ trace_live ioa s t
+  .
+
+  Definition trace_valid
+    (ioa : IOA action_t)
+    (t : trace_t action_t)
+    : Prop :=
+    exists s : ioa.(state_t),
+      ioa.(initial) s /\ trace_correct ioa (Some s) t
+  .
+
+  (*
+    The composition of two automata is
+    simply the composition of the functions
+   *)
+
+  (*
+    T?*T'?
+   *)
+  Definition option_prod_t (T T' : Type) : Type := (option T)*(option T').
+
+  (*
+    (T*T')?
+   *)
+  Definition quotient_t (T T' : Type) : Type := option (T*T').
+
+  (*
+    This function is a quotient for the
+    equivalence relation which merges the
+    None value on the set (option T, option T')
+   *)
+  Definition quotient_option
+    {T T' : Type}
+    (p : option_prod_t T T')
+    : quotient_t T T' :=
+    match p with
+      | (Some va, Some vb) => Some (va, vb)
+      | _ => None
+    end
+  .
+
+  Hint Unfold quotient_option : ioa.
+
+  (*Notation "( a , b ) ~>" := (quotient_option a b).*)
+  Notation "a ~>" := (quotient_option a) (at level 1).
+
+  Definition ioa_composition
+    (ioaA ioaB : IOA action_t)
+    : IOA action_t :=
+    mkIOA
+      _
+      (ioaA.(state_t) * ioaB.(state_t))
+      (sig_composition ioaA.(sig) ioaB.(sig))
+      (fun s => ioaA.(initial) (fst s) /\ ioaB.(initial) (snd s))
+      (
+        fun s a =>
+          ((ioaA.(transition) (fst s) a),
+            (ioaB.(transition) (snd s) a)) ~>
+      )
+      (sig_composition_dec ioaA.(act_dec) ioaB.(act_dec))
+  .
+
+  Notation "a /*/ b" := (ioa_composition a b) (at level 50).
+
+  Definition prod_state_t
+    (ioaA ioaB : IOA action_t)
+    : Type :=
+    option_prod_t ioaA.(state_t) ioaB.(state_t).
+
+  Definition quotient_state_t
+    (ioaA ioaB : IOA action_t)
+    : Type :=
+    quotient_t ioaA.(state_t) ioaB.(state_t).
+
+  Variable ioaA ioaB : IOA action_t.
+
+  (*
+    A fondamental lemma is that the monad
+    'descent au quotient'
+   *)
+
+  Lemma monad_compat_with_quotient_option :
+    forall a : action_t,
+    forall (s : prod_state_t ioaA ioaB),
+      monad (ioaA /*/ ioaB) s~> a =
+        ( (monad ioaA (fst s) a), (monad ioaB (snd s) a) )~>
+  .
+  Proof.
+    intros.
+    destruct s as (sA, sB).
+    unfold
+      monad,
+      ioa_composition,
+      quotient_option.
+    simpl.
+    destruct sA, sB ; auto.
+    destauto ; auto.
+  Qed.
+
+  (*
+    The lemma is extendible to traces
+   *)
+  Lemma execute_trace_compat_with_quotient_option :
+    forall t :  trace_t action_t,
+    forall (s : prod_state_t ioaA ioaB),
+      [ioaA /*/ ioaB] s~> >-> t =
+        ( ([ioaA] (fst s) >-> t), ([ioaB] (snd s) >-> t) ) ~>
+  .
+  Proof.
+    induction t.
+    - destruct s. auto.
+    - intros. simpl.
+      rewrite monad_compat_with_quotient_option.
+      auto.
+  Qed.
+
+  (*
+    And we can then deduce the equivalence on
+    enabled actions and traces
+   *)
+
+  Lemma action_enabled_compat_with_quotient_option :
+    forall a : action_t,
+    forall (s : prod_state_t ioaA ioaB),
+      action_enabled (ioaA /*/ ioaB) s~> a <->
+        (action_enabled ioaA (fst s) a) /\ (action_enabled ioaB (snd s) a)
+  .
+  Proof.
+    intros.
+    unfold action_enabled.
+    rewrite monad_compat_with_quotient_option.
+    unfold quotient_option.
+    repeat (simpl_match ; auto) ;
+      split ; intro HH ; try discriminate ; auto ; try split ; try discriminate ; destruct HH ; auto.
+  Qed.
+
+  Lemma trace_enabled_compat_with_quotient_option :
+    forall t : trace_t action_t,
+    forall (s : prod_state_t ioaA ioaB),
+      trace_enabled (ioaA /*/ ioaB) s~> t <->
+        (trace_enabled ioaA (fst s) t) /\ (trace_enabled ioaB (snd s) t)
+  .
+  Proof.
+    intros.
+    unfold trace_enabled.
+    rewrite execute_trace_compat_with_quotient_option.
+    unfold quotient_option.
+    repeat (simpl_match ; auto) ;
+      split ; intro HH ; try discriminate ; auto ; try split ; try discriminate ; destruct HH ; auto.
+  Qed.
+
+  (*
+    Also extend liveness
+
+    From now on, we also need decidability
+    on actions because we need to know if
+    the action is local or not
+
+    Note : it is only possible to extend
+    liveness on an enabled trace because
+    we don't want the last state to be
+    not None. Therefore we directly prove
+    the compatibility of :
+
+          enabled + live = correct
+
+    traces.
+
+    Note 2 : we also need hypothesis
+    on input enabled automata. The
+    reason for that is that we need
+    to have the validity of the next
+    in case of enabled output action.
+   *)
+
+  Definition input_enabled (ioa : IOA action_t) : Prop :=
+    forall a : action_t,
+      In _ (input ioa.(sig)) a ->
+      forall s, action_enabled ioa s a.
+
+  Definition action_coherent (ioa : IOA action_t) : Prop :=
+    forall a : action_t,
+      ~In _ (acts ioa.(sig)) a ->
+      forall s, monad ioa s a = s.
+
+  Definition ioa_compatible (ioaA ioaB : IOA action_t) : Prop :=
+    Disjoint _ (local ioaA.(sig)) (local ioaB.(sig)).
+
+  (*
+    If the two sub-traces are correct, then the global
+    trace also is. This result doesn't need any assumptions,
+    so we put it here.
+   *)
+
+  Lemma traces_correct_then_composition_correct :
+    forall t : trace_t action_t,
+    forall (sA : option ioaA.(state_t)) (sB : option ioaB.(state_t)),
+      (trace_correct ioaA sA t) /\ (trace_correct ioaB sB t) ->
+      trace_correct (ioaA /*/ ioaB) (sA, sB)~> t.
+  Proof.
+    unfold trace_correct.
+    intros * [[HAen HAlive] [HBen HBlive]].
+    destruct sA, sB.
+    - split.
+      + apply trace_enabled_compat_with_quotient_option. auto.
+      + unfold trace_live in *.
+        intros.
+        intro.
+        rewrite execute_trace_compat_with_quotient_option in H0.
+        apply action_enabled_compat_with_quotient_option in H0.
+        destruct H ; destruct H.
+        * assert (In action_t (local (sig ioaA)) x).
+          apply intern_in_local. auto.
+          apply HAlive in H1.
+          tauto.
+        * assert (In action_t (local (sig ioaB)) x).
+          apply intern_in_local. auto.
+          apply HBlive in H1.
+          tauto.
+        * assert (In action_t (local (sig ioaA)) x).
+          apply output_in_local. auto.
+          apply HAlive in H1.
+          tauto.
+        * assert (In action_t (local (sig ioaB)) x).
+          apply output_in_local. auto.
+          apply HBlive in H1.
+          tauto.
+    - simpl.
+      assert (~trace_enabled ioaB None t).
+      auto with ioa.
+      contradiction.
+    - simpl.
+      assert (~trace_enabled ioaA None t).
+      auto with ioa.
+      contradiction.
+    - simpl.
+      assert (~trace_enabled ioaB None t).
+      auto with ioa.
+      contradiction.
+  Qed.
+
+
+
+  (*
+    TODO:
+    Might be possible to use
+    lighter hypothesis like :
+    acts_dec instead of sig_dec
+
+    Note : removed as we enforced the decidability in the def
+   *)
+  (*
+  Hypothesis HioaA_sig_dec :
+    sig_dec ioaA.(sig).
+  Hypothesis HioaB_sig_dec :
+    sig_dec ioaB.(sig).*)
+
+  Hypothesis HioaA_input_enabled :
+    input_enabled ioaA.
+  Hypothesis HioaB_input_enabled :
+    input_enabled ioaB.
+
+  Hypothesis HioaA_coherent :
+    action_coherent ioaA.
+  Hypothesis HioaB_coherent :
+    action_coherent ioaB.
+
+  Hypothesis Hioa_compatible :
+    ioa_compatible ioaA ioaB.
+
+  Lemma trace_correct_compat_with_quotient_option :
+    forall t : trace_t action_t,
+    forall (sA : option ioaA.(state_t)) (sB : option ioaB.(state_t)),
+      trace_correct (ioaA /*/ ioaB) (sA, sB)~> t <->
+        (trace_correct ioaA sA t) /\ (trace_correct ioaB sB t)
+  .
+  Proof.
+    intros.
+    split.
+    - intro.
+      split.
+      + unfold trace_correct.
+        split.
+        * destruct H.
+          apply trace_enabled_compat_with_quotient_option in H. apply H.
+        * destruct H.
+          apply trace_enabled_compat_with_quotient_option in H.
+          destruct H.
+          unfold trace_live in *.
+          intros.
+          unfold action_enabled.
+          case_eq (monad ioaA ([ioaA] sA >-> t) a).
+          {
+            intros.
+            (* because the action is None, one of them is none *)
+            (* in this case, it is B *)
+            case_eq (monad ioaB ([ioaB] sB >-> t) a) ; intros.
+
+            eapply sig_composition_keep_local in H2.
+            apply H0 in H2.
+            rewrite execute_trace_compat_with_quotient_option in H2.
+            contradict H2.
+            apply action_enabled_compat_with_quotient_option.
+            simpl. unfold action_enabled. rewrite H3, H4.
+            split ; discriminate.
+            edestruct sig_act_dec.
+            apply ioaB.(act_dec).
+            Unshelve. 3: apply a.
+
+            (* if a is an action of B *)
+            rewrite act_to_local_input in H5.
+            destruct H5.
+
+            (* if a is in local B *)
+            unfold ioa_compatible in *.
+            destruct Hioa_compatible.
+            specialize H6 with x.
+            contradict H6.
+            unfold In.
+            apply Intersection_intro ; auto.
+
+            (* if a is in input B *)
+            apply HioaB_input_enabled in H5.
+            specialize H5 with ([ioaB] sB >-> t).
+            contradiction.
+
+            (* if a is not an action of B *)
+            unfold action_coherent in *.
+            eapply HioaB_coherent in H5.
+            rewrite H5 in H4.
+            unfold trace_enabled in H1.
+            contradiction.
+          }
+          {
+            auto.
+          }
+      + unfold trace_correct.
+        split.
+        * destruct H.
+          apply trace_enabled_compat_with_quotient_option in H. apply H.
+        * destruct H.
+          apply trace_enabled_compat_with_quotient_option in H.
+          destruct H.
+          unfold trace_live in *.
+          intros.
+          unfold action_enabled.
+          case_eq (monad ioaB ([ioaB] sB >-> t) a).
+          {
+            intros.
+            (* because the action is None, one of them is none *)
+            (* in this case, it is B *)
+            case_eq (monad ioaA ([ioaA] sA >-> t) a) ; intros.
+
+            eapply sig_composition_keep_local in H2.
+            rewrite sig_composition_commute in H2.
+            apply H0 in H2.
+            rewrite execute_trace_compat_with_quotient_option in H2.
+            contradict H2.
+            apply action_enabled_compat_with_quotient_option.
+            simpl. unfold action_enabled. rewrite H3, H4.
+            split ; discriminate.
+            edestruct sig_act_dec.
+            apply ioaA.(act_dec).
+            Unshelve. 3: apply a.
+
+            (* if a is an action of B *)
+            rewrite act_to_local_input in H5.
+            destruct H5.
+
+            (* if a is in local B *)
+            unfold ioa_compatible in *.
+            destruct Hioa_compatible.
+            specialize H6 with x.
+            contradict H6.
+            unfold In.
+            apply Intersection_intro ; auto.
+
+            (* if a is in input B *)
+            apply HioaA_input_enabled in H5.
+            specialize H5 with ([ioaA] sA >-> t).
+            contradiction.
+
+            (* if a is not an action of B *)
+            unfold action_coherent in *.
+            eapply HioaA_coherent in H5.
+            rewrite H5 in H4.
+            unfold trace_enabled in H1.
+            contradiction.
+          }
+          {
+            auto.
+          }
+    - apply traces_correct_then_composition_correct.
+  Qed.
+
+  (*
+    After this main theorem, we can continue with
+    creating tools for the compositions of more
+    automata easily
+   *)
+
+  (*
+    "Identity" automata.
+    It is not an actual identity in the sence of equality
+    but we will prove later that a /*/ id ~ id /*/ a ~ a
+    where ~ is a relation of bisimulation (with a very specific def)
+    between the two automata.
+   *)
+
+  Definition ioa_neutral
+    : IOA action_t.
+    refine (
+        mkIOA
+          _
+          unit
+          (empty_sig action_t)
+          (fun s => True)
+          (fun s a => Some s)
+          _
+      )
+    .
+    unfold sig_dec, empty_sig.
+    simpl. intro.
+    repeat split ; right ; unfold In ; intro H ; destruct H.
+  Defined.
+
+  Fixpoint ioa_composition_list
+    (l : list (IOA action_t))
+    : IOA action_t :=
+    match l with
+      | nil => ioa_neutral
+      | a::nil => a
+      | a::t => a /*/ (ioa_composition_list t)
+    end.
+End IOA.
+
+Notation "[ ioa ] s >-> t" := (execute_trace ioa s t) (at level 70).
+Notation "a ~>" := (quotient_option a) (at level 1).
+Notation "a /*/ b" := (ioa_composition a b) (at level 50).
+
+Section Simulation.
+  (*
+    Definition of abstraction, refinement, and simulation relations
+   *)
+
+  (*
+    Hiding some actions
+   *)
+  Definition
+    hide
+      {action_t : Type}
+      (ioa : IOA action_t)
+      (p : Ensemble action_t)
+    : IOA action_t.
+    refine (
+    mkIOA
+      _
+      ioa.(state_t)
+      (sig_hide ioa.(sig) p)
+      ioa.(initial)
+      ioa.(transition)
+      _
+    ).
+    unfold sig_dec, sig_hide.
+    simpl. intro.
+    split ; [|split].
+    -
+
+  Fixpoint
+    filter
+      {action_t : Type}
+      (sig : Signature action_t)
+      (act_dec : act_dec_t sig)
+      (t : trace_t action_t)
+    : trace_t action_t :=
+    match t with
+      | nil => nil
+      | a::t' =>
+          if act_dec a then
+            a::(@filter _ sig act_dec t')
+          else
+            @filter _ sig act_dec t'
+    end.
+
+  (*
+    I want to define a definition of simulation specific to IOA.
+    The reason for that is that it make it easier to reason about it.
+
+    A simulation H from A to B is a function that associate each :
+    - output action of A to an output action of B
+    - input action of A to an input action of B
+    - for every state s and every external action enabled in
+      automata A, H(a) is also enabled in B
+
+
+    There are mainly three ways to define a partial function :
+    1. either the monad Option
+    2. either using specification ({ x | P })
+    3. either using a dummy for the value we are interested in
+
+    The option 2. is very complex to manipulate so we prefer to avoid.
+    Therefore we are left with option 1. and 3.
+
+    I decided to go for option 3. as it makes it easier to manipulate
+    and is just enough for all the proof, the only downside is when defining
+    the simulation function, it can be a bit disrupting at first.
+   *)
+
+  Definition
+    simulation_t
+    :=
+    fun a b : Type => a -> b
+  .
+
+  Definition
+    simulation_spec
+      {action_A_t action_B_t : Type}
+      (ioaA : IOA action_A_t)
+      (ioaB : IOA action_B_t)
+      (S : simulation_t action_A_t action_B_t)
+    : Prop :=
+    forall a : action_A_t,
+      (
+        In _ (input ioaA.(sig)) a ->
+        In _ (input ioaB.(sig)) (S a)
+      )
+      /\ (
+        In _ (output ioaA.(sig)) a ->
+        In _ (output ioaB.(sig)) (S a)
+      )
+  .
+
+  Lemma
+    simulation_spec_refl :
+    forall T : Type,
+    forall ioa : IOA T,
+      simulation_spec ioa ioa (fun a => a)
+  .
+  Proof.
+    intros.
+    unfold simulation_spec.
+    auto.
+  Qed.
+
+  Lemma simulation_spec_trans :
+    forall TA TB TC : Type,
+    forall ioaA : IOA TA, forall ioaB : IOA TB, forall ioaC : IOA TC,
+    forall S : simulation_t TA TB,
+    forall S': simulation_t TB TC,
+      simulation_spec ioaA ioaB S ->
+      simulation_spec ioaB ioaC S' ->
+      simulation_spec ioaA ioaC (fun a => S' (S a))
+  .
+  Proof.
+    intros.
+    unfold simulation_spec in *.
+    intro.
+    split ; intro ; apply H0 ; apply H ; auto.
+  Qed.
+
+  Fixpoint
+    simulate
+      {action_A_t action_B_t : Type}
+      (S : simulation_t action_A_t action_B_t)
+      (t : trace_t action_A_t)
+      : trace_t action_B_t :=
+    match t with
+      | nil => nil
+      | a::t' =>
+          (S a)::(simulate S t')
+    end
+  .
+
+  Definition
+    simulation
+      {action_A_t action_B_t : Type}
+      (ioaA : IOA action_A_t)
+      (ioaB : IOA action_B_t)
+      (S : simulation_t action_A_t action_B_t)
+      (act_A_dec : act_dec_t ioaA.(sig))
+      (act_B_dec : act_dec_t ioaB.(sig))
+    : Prop :=
+    simulation_spec ioaA ioaB S /\
+      forall t : trace_t action_A_t,
+        trace_valid ioaA t ->
+        exists t' : trace_t action_B_t,
+          trace_valid ioaB t' /\
+            simulate S (filter act_A_dec t) = filter act_B_dec t'
+  .
+
+  Lemma
+    simulation_refl :
+    forall T : Type,
+    forall ioa : IOA T,
+    forall act_dec : act_dec_t ioa.(sig),
+      simulation ioa ioa (fun a => a) act_dec act_dec
+  .
+  Proof.
+    intros.
+    unfold simulation.
+    split.
+    - apply simulation_spec_refl.
+    - intros.
+      exists t. split ; auto.
+      clear H.
+      induction t ; auto.
+      simpl.
+      simpl_match. rewrite IHt. auto.
+      auto.
+  Qed.
+
+  Lemma
+    simulation_trans :
+    forall TA TB TC : Type,
+    forall ioaA : IOA TA, forall ioaB : IOA TB, forall ioaC : IOA TC,
+    forall act_A_dec : act_dec_t ioaA.(sig),
+    forall act_B_dec : act_dec_t ioaB.(sig),
+    forall act_C_dec : act_dec_t ioaC.(sig),
+    forall S : simulation_t TA TB,
+    forall S': simulation_t TB TC,
+      simulation ioaA ioaB S act_A_dec act_B_dec ->
+      simulation ioaB ioaC S' act_B_dec act_C_dec ->
+      simulation ioaA ioaC (fun x => S' (S x)) act_A_dec act_C_dec
+  .
+  Proof.
+    intros.
+    unfold simulation in *.
+    split.
+    - eapply simulation_spec_trans.
+      apply H.
+      apply H0.
+    - intros.
+      destruct H as [_ H].
+      destruct H0 as [_ H0].
+      specialize H with t.
+      apply H in H1. clear H. destruct H1 as [t_tmp [H1 H]].
+      specialize H0 with t_tmp.
+      apply H0 in H1. clear H0.
+      destruct H1 as [t' [H1 H0]].
+      exists t'. split ; auto.
+      rewrite <-H in H0.
+      rewrite <-H0.
+      clear H H0.
+      induction t ; auto.
+      simpl ; simpl_match ; rewrite IHt ; auto.
+  Qed.
+  
+  Definition
+    bisimulation
+      {action_A_t action_B_t : Type}
+      (ioaA : IOA action_A_t)
+      (ioaB : IOA action_B_t)
+      (S : simulation_t action_A_t action_B_t)
+      (S__inv : simulation_t action_B_t action_A_t)
+      (act_A_dec : act_dec_t ioaA.(sig))
+      (act_B_dec : act_dec_t ioaB.(sig))
+    : Prop :=
+    simulation ioaA ioaB S act_A_dec act_B_dec /\
+      simulation ioaB ioaA S__inv act_B_dec act_A_dec /\
+      (forall a, S (S__inv a) = a) /\ (forall b, S__inv (S b) = b)
+  .
+
+  Lemma
+    bisimulation_commute :
+    forall TA TB : Type,
+    forall ioaA : IOA TA, forall ioaB : IOA TB, forall S S__inv act_A_dec act_B_dec,
+      bisimulation ioaA ioaB S S__inv act_A_dec act_B_dec ->
+      bisimulation ioaB ioaA S__inv S act_B_dec act_A_dec
+  .
+  Proof.
+    unfold bisimulation.
+    intros.
+    split ; [ | split].
+    - unfold simulation in *.
+      destruct H as [_ [H _]].
+      split.
+      + destruct H as [H _].
+        unfold simulation_spec in *.
+        intro.
+        split ; intro ; apply H ; auto.
+      + apply H.
+    - destruct H as [H _].
+      unfold simulation in *.
+      split.
+      + destruct H as [H _].
+        unfold simulation_spec in *.
+        intro.
+        split ; intro ; apply H ; auto.
+      + apply H.
+    - intros ; split ; apply H ; auto.
+  Qed.
+
+  Definition
+    ioa_equivalent
+      {action_A_t action_B_t : Type}
+      (ioaA : IOA action_A_t)
+      (ioaB : IOA action_B_t)
+      (act_A_dec : act_dec_t ioaA.(sig))
+      (act_B_dec : act_dec_t ioaB.(sig))
+    : Prop :=
+    exists S S__inv,
+      bisimulation ioaA ioaB S S__inv act_A_dec act_B_dec.
+
+  (*
+    Bisimulation is an equivalence relation
+   *)
+  Lemma
+    ioa_refl :
+    forall T : Type,
+    forall ioa : IOA T,
+    forall act_dec : act_dec_t ioa.(sig),
+      ioa_equivalent ioa ioa act_dec act_dec
+  .
+  Proof.
+    intros.
+    exists (fun a => a), (fun a => a).
+    unfold bisimulation.
+    split ; [|split].
+    - apply simulation_refl.
+    - apply simulation_refl.
+    - auto.
+  Qed.
+
+  Lemma
+    ioa_sym :
+    forall TA TB : Type,
+    forall ioaA : IOA TA, forall ioaB : IOA TB,
+    forall act_A_dec : act_dec_t ioaA.(sig),
+    forall act_B_dec : act_dec_t ioaB.(sig),
+      ioa_equivalent ioaA ioaB act_A_dec act_B_dec ->
+        ioa_equivalent ioaB ioaA act_B_dec act_A_dec
+  .
+  Proof.
+    unfold ioa_equivalent.
+    intros.
+    destruct H.
+    destruct H.
+    exists x0, x.
+    unfold bisimulation in *.
+    split ; [ |split ] ; try apply H.
+    intros. split ; apply H ; auto.
+  Qed.
+
+  Lemma
+    ioa_transitive :
+    forall TA TB TC : Type,
+    forall ioaA : IOA TA, forall ioaB : IOA TB, forall ioaC : IOA TC,
+    forall act_A_dec : act_dec_t ioaA.(sig),
+    forall act_B_dec : act_dec_t ioaB.(sig),
+    forall act_C_dec : act_dec_t ioaC.(sig),
+      ioa_equivalent ioaA ioaB act_A_dec act_B_dec ->
+        ioa_equivalent ioaB ioaC act_B_dec act_C_dec ->
+        ioa_equivalent ioaA ioaC act_A_dec act_C_dec
+  .
+  Proof.
+    intros.
+    unfold ioa_equivalent in *.
+    destruct H.
+    destruct H.
+    destruct H0.
+    destruct H0.
+    exists (fun a => x1 (x a)), (fun a => x0 (x2 a)).
+    unfold bisimulation in *.
+    split ; [|split].
+    - eapply simulation_trans.
+      apply H.
+      apply H0.
+    - eapply simulation_trans.
+      apply H0. apply H.
+    - intros.
+      destruct H0 as [_ [_ [Ha0 Hb0]]].
+      destruct H as [_ [_ [Ha Hb]]].
+      split.
+      + intros. rewrite Ha. auto.
+      + intros. rewrite Hb0. auto.
+  Qed.
+
+  (*
+    It means that we can define a quotient over the set of IOA.
+    In particular, this quotient is compatible with the product operation :
+                  /*/
+      IOA*IOA -----------> IOA
+        |                   |
+        |                   |
+Q_~*Q_~ |                   | Q_~
+        |                   |
+        v                   v
+   IOA/~*IOA/~ ---------> IOA/~
+                /*/
+
+    Or, equivalently, that every equivalent pairs of ioa, when composed,
+    gives equivalent ioa
+   *)
+
+  Lemma
+    composition_compat_with_equiv :
+    forall T T' : Type,
+    forall ioaA ioaB : IOA T,
+    forall ioaA' ioaB' : IOA T',
+    forall act_A_dec : act_dec_t ioaA.(sig),
+    forall act_A'_dec : act_dec_t ioaA'.(sig),
+    forall act_B_dec : act_dec_t ioaB.(sig),
+
+      ioa_equivalent ioaA ioaA'
+
+  (*
+    Now we can talk about the identity ioa defined above.
+    If we compose with this operator, we are
+   *)
+
+  
+  (*
+  The goals are :
+  - Tying to make composition as easy as possible
+  - Proving result on simulation and making good definitions
+  - Adding fairness and results to make it easier to reason about it
+  - making reasonning about temporality easier
+   *)
+
+  (* ---------------------------------------------------------------
+
+   We first defines some basic definitions on the execution of an IOA
+
+   --------------------------------------------------------------- *)
+
+  (* A section is a tripplet (state, action, state) *)
+
+  Definition section_t : Type := ioa.(state_t) * actions_t * ioa.(state_t).
+
+  Definition is_section (sect : section_t) : Prop :=
+    let '(s, a, s') := sect in
+    ioa.(transition) s a = Some s'.
+
+  (* A fragment of execution defines the type used to represent the traces *)
+  Definition fragment_t : Type := nat -> section_t.
+
+  (* check if the states are matching from one to the next *)
+  Definition is_fragment (f : fragment_t) : Prop :=
+    forall i : nat,
+      let '(_, _, s) := (f i) in
+      let '(s', _, _) := (f (i+1)) in
+      s = s'.
+
+  (* Check if each sections are section of execution *)
+  Definition is_exec (f : fragment_t) : Prop :=
+    forall i : nat, is_section (f i).
+
+  (* A trace is a fragment which is an execution *)
+  Definition is_trace (t : fragment_t) : Prop :=
+    is_fragment t /\ is_exec t.
+
+  (* ---------------------------------------------------------------
+
+   Then we definine what is the composition of automata
+
+   --------------------------------------------------------------- *)
+
+  (* A composition is construct around a type, so that it is easiser
+     to manipulate in proofs *)
+  Definition composer_t (t : Type) : Type := t -> IOA actions_t.
+
+  Definition composition {t : Type} (c : composer_t t) : IOA actions_t :=
+    mkIOA
+      _
+
+  .
